cancellation/Cancellation.v
@@ -1,7 +1,7 @@
 Require Import Coqlib.
 Require Import Behavior.
 Require Import AList.
-Require Import SMod2HMod SMod2HModElim.
+Require Import SMod2HMod SMod2HModAux.
 Require Import Skeleton.
 Require Import PCM IPM.
 Require Import Any.
@@ -9,94 +9,19 @@ Require Export STB.
 Require Import ModSim ISim HPSim.
 Require Import CtxRefine CtxRefineFacts MainAdequacy ClosedAdequacy.
 Require Import SimGlobal SimGlobalFacts.
-Require Import Cancel.
 Require Import SMod HMod Mod Events.
+Require Import HModInline Cancel ElimRel.
+Require Import Mod2ITree StRed.
 
 Set Implicit Arguments.
 
-
-Module StRed.
-Section RED.
-
-  Lemma interp_bind
-        A B
-        (itr: itree (stateE +' coreE) A)
-        (ktr: A -> itree (stateE +' coreE) B)
-        st0
-    :
-      interp_stateE B (v <- itr ;; ktr v) st0 =
-      '(st1, v) <- interp_stateE A (itr) st0 ;; interp_stateE B (ktr v) st1.
-  Proof.
-    unfold interp_stateE. grind. destruct x. grind.
-  Qed.
-
-  Lemma interp_tau
-        A (itr: itree (stateE +' coreE) A)
-        st0 
-    :
-      interp_stateE _ (tau;; itr) st0 = tau;; interp_stateE _ itr st0
-  .
-  Proof. 
-    unfold interp_stateE. grind. 
-  Qed.
-
-  Lemma interp_st
-        E st0 T e
-    :
-      @interp_stateE E T (trigger e) st0 =
-      '(st1, r) <- handle_stateE _ e st0;;
-      tau;; Ret (st1, r).
-  Proof.
-    unfold interp_stateE. grind. destruct x. grind.
-  Qed.
-
-  Lemma interp_ret
-        E A st0 v
-    :
-      @interp_stateE E A (Ret v) st0 = Ret (st0, v)
-  .
-  Proof. 
-    unfold interp_stateE. grind.
-  Qed.
-  
-  Lemma interp_core
-        st0 T
-        (e: coreE T)
-    :
-      @interp_stateE (coreE) _ (trigger e) st0 = r <- trigger e;; tau;; Ret (st0, r)
-  .
-  Proof.
-    unfold interp_stateE. grind.
-    unfold Mod2STS.pure_state. grind.
-  Qed.
-
-  Lemma interp_UB
-        st0 A
-    :
-      (@interp_stateE (stateE +' coreE) A (triggerUB) st0) = triggerUB
-  .
-  Proof.
-    unfold interp_stateE, Mod2STS.pure_state, triggerUB. grind.
-  Qed.
-  
-  Lemma interp_NB
-        st0 A
-    :
-      (@interp_stateE (stateE +' coreE) A (triggerNB) st0) = triggerNB
-  .
-  Proof.
-    unfold interp_stateE, Mod2STS.pure_state, triggerNB. grind.
-  Qed.  
-
-End RED.
-End StRed.
 
 Section CANCEL.
   Context `{Σ: GRA.t}.
   Variable ginv: Sk.t -> invspec.
   Variable stb: Sk.t -> gname -> option fspec.
-
   Variable md: SMod.t.
+  Notation iProp := (iProp Σ).
 
   Let sk: Sk.t := SMod.sk md.
   Let ms (sk0: Sk.t) (SKINCL: incl sk sk0) (SKWF: Sk.wf sk0) := 
@@ -116,680 +41,11 @@ Section CANCEL.
       fn (FIND: alist_find fn (_stb SKINCL SKWF) = None),
       (<<NONE: stb sk0 fn = None>>).
 
-  Lemma stb_in_alist_find
-        sk0 fn fsp
-        (SKINCL: incl sk sk0) 
-        (SKWF: Sk.wf sk0)
-        (SOME: stb sk0 fn = Some fsp)
-      :
-        exists l fbody, 
-          alist_find fn (SModSem.fnsems (SMod.modsem md sk0)) = Some (l, {|fsb_fspec :=fsp; fsb_body := fbody|}).
-  Proof.
-    destruct (alist_find fn (_stb SKINCL SKWF)) eqn: FIND; cycle 1.
-    { eapply STBSOUND in FIND. des. clarify. }
-    unfold _stb, sbtb, ms in FIND.
-    rewrite/__ alist_find_map_snd/o_map in FIND. des_ifs.
-    destruct p0, f. exists l, fsb_body. repeat f_equal.
-    assert (alist_find fn (_stb SKINCL SKWF) = Some (l, fsb_fspec)).
-    { rewrite/_stb alist_find_map_snd /o_map /sbtb /ms Heq. ss. }
-    eapply STBCOMPLETE in H. ss. rewrite SOME in H. inv H. ss.
-  Qed.
-
-  Lemma fsb_find_spec fn l fsp fbody sk0
-    (SKINCL: incl sk sk0) 
-    (SKWF: Sk.wf sk0) 
-    (FIND: alist_find fn (sbtb SKINCL SKWF) = Some (l, {|fsb_fspec := fsp; fsb_body := fbody|}))
-  :
-    alist_find fn (_stb SKINCL SKWF) = Some (l, fsp).
-  Proof.
-    unfold sbtb, _stb.
-    rewrite/__ alist_find_map_snd/o_map FIND. ss.
-  Qed. 
-
-  Lemma stb_find_fsb fn fsp l fspec fbody sk0
-    (SKINCL: incl sk sk0) 
-    (SKWF: Sk.wf sk0) 
-    (STB: stb sk0 fn = Some fsp)
-    (FIND: alist_find fn (sbtb SKINCL SKWF) = Some (l, {|fsb_fspec:= fspec; fsb_body := fbody|}))
-  :
-    fsp = fspec.
-  Proof.
-    specialize (STBCOMPLETE SKINCL SKWF fn).
-    eapply fsb_find_spec, STBCOMPLETE in FIND. ss.
-    rewrite FIND in STB. inv STB. ss. 
-  Qed.
-
-  Let md_elim: HMod.t := HModAux.to_elimI (SModElim.to_elim md). 
-  Let md_tgt: HMod.t := HModAux.to_elimI (SMod.to_hmod ginv stb md).
+  Let md_src: HMod.t := HModAux.inline (SModAux.to_hmod md). 
+  Let md_tgt: HMod.t := HModAux.inline (SMod.to_hmod ginv stb md).
   
-  Let ms_elim: HModSem.t := HMod.modsem md_elim (md_elim.(HMod.sk)).
+  Let ms_src: HModSem.t := HMod.modsem md_src (md_src.(HMod.sk)).
   Let ms_tgt: HModSem.t := HMod.modsem md_tgt (md_tgt.(HMod.sk)).
-
-  (* Sk.t lemmas *)
-  (* sk0: list (string * Any.t) *)
-  (* SKINCL: incl (SMod.sk md) sk0 *)
-  (* SKWF: Sk.wf sk0 *)
-
-  Definition hmod_elim_head X P : Any.t -> itree hmodE ((nat * X * nat * X) * Any.t)
-    :=
-    fun varg =>
-      my_tid <- trigger Tid;; tau;;
-      x <- trigger (Choose X);; tau;;
-      arg <- trigger (Choose Any.t);; tau;;
-      trigger (Guarantee (P my_tid x varg arg));;; tau;; tau;;
-      my_tid' <- trigger Tid;; tau;;
-      x' <- trigger (Take X);; tau;;
-      varg' <- trigger (Take _);; tau;;
-      trigger (Assume (P my_tid' x' varg' arg));;; tau;;
-      Ret ((my_tid, x, my_tid', x'), varg').
-
-  Definition hmod_elim_tail X Q : (nat * X * nat * X) -> Any.t -> itree hmodE Any.t
-    :=
-    fun '(my_tid, x, my_tid', x') vret' =>
-      ret <- trigger (Choose Any.t);; tau;;
-      trigger (Guarantee (Q my_tid' x' vret' ret));;; tau;; tau;; tau;;
-      vret <- trigger (Take Any.t);; tau;;
-      trigger (Assume (Q my_tid x vret ret));;; tau;;
-      Ret vret.
-      
-  Definition HoareSpawnE ginv' (fsp: fspec) (fn: gname) (arg: Any.t) : itree hmodE nat :=
-    x <- trigger (Choose fsp.(meta));; tau;;
-    varg <- trigger (Choose Any.t);; tau;;
-    tid <- trigger (Spawn fn arg);; tau;;
-    trigger (Guarantee (ginv' tid -∗ fsp.(precond) tid x arg varg));;; tau;;
-    Ret tid.
-
-  Definition HoareYieldE ginv' (tid: nat) : itree hmodE unit :=
-    trigger (Guarantee (ginv' tid));;; tau;;
-    trigger (Yield tid);;; tau;;
-    my_tid <- trigger Tid;; tau;;
-    trigger (Assume (ginv' my_tid)).
-
-  (*** use interp_hpI ***) 
-  Variant elim_rel_def
-    (relc: forall X Y (RR: X -> Y -> Prop), bool -> itree hmodE X -> itree hmodE Y -> Prop)
-    {X Y}
-    (RR: X -> Y -> Prop)
-    (reli: bool -> itree hmodE X -> itree hmodE Y -> Prop)
-    : bool -> itree hmodE X -> itree hmodE Y -> Prop
-  :=
-  | elim_rel_base v0 v1 p
-    (RET: RR v0 v1)
-    :
-    elim_rel_def relc RR reli p (Ret v0) (Ret v1)
-
-  | elim_rel_tau_src p itrS itrT
-      (ITR: reli true itrS itrT)
-    :
-    elim_rel_def relc RR reli p (tau;; itrS) (itrT)
-
-  | elim_rel_tau_tgt p itrS itrT
-      (ITR: reli true itrS itrT)
-    :
-    elim_rel_def relc RR reli p (itrS) (tau;; itrT)
-
-  | elim_rel_add {R} p itr ktrS ktrT
-      (KTR: forall (v: R), reli true (ktrS v) (ktrT v))
-    :
-    elim_rel_def relc RR reli p (itr >>= ktrS) (itr >>= ktrT)
-
-  | elim_rel_head X P p v src tgt ktrS ktrT
-      (KTR: forall m, reli true (ktrS v) (ktrT (m, v)))
-      (EQS: src = ktrS v)
-      (EQT: tgt = (@hmod_elim_head X P v) >>= ktrT)
-    :
-    elim_rel_def relc RR reli p src tgt
-                  
-  | elim_rel_tail X Q m v p src tgt ktrS ktrT
-      (KTR: reli true (ktrS v) (ktrT v))
-      (EQS: src = ktrS v)
-      (EQT: tgt = (@hmod_elim_tail X Q m v) >>= ktrT)
-    :
-    elim_rel_def relc RR reli p src tgt
-
-  | elim_rel_NB
-      p src tgt itrS ktrT
-      (EQS: src = itrS)
-      (EQT: tgt = trigger (Choose void) >>= ktrT)
-    :
-    elim_rel_def relc RR reli p src tgt
-
-   | elim_rel_spawn
-      sk0 p src tgt f fn args ktrS ktrT
-      (SKINCL: incl sk sk0)
-      (SKWF: Sk.wf sk0)
-      (STB: stb sk0 fn = Some f)
-      (KTR: forall x, reli true (ktrS x) (ktrT x))
-      (EQS: src =  trigger (Spawn fn args) >>= ktrS)
-      (EQT: tgt = HoareSpawnE (ginv sk0) f fn args >>= ktrT)
-    :
-    elim_rel_def relc RR reli p src tgt
-
-  | elim_rel_yield
-      sk0 tid p src tgt ktrS ktrT
-      (SKINCL: incl sk sk0)
-      (SKWF: Sk.wf sk0)
-      (KTR: forall x, reli true (ktrS x) (ktrT x))
-      (EQS: src = trigger (Yield tid) >>= ktrS)
-      (EQT: tgt = HoareYieldE (ginv sk0) tid >>= ktrT)
-    :
-    elim_rel_def relc RR reli p src tgt
-
-  | elim_rel_progress
-      src tgt
-      (REL: relc X Y RR false src tgt)
-    :
-    elim_rel_def relc RR reli true src tgt 
-  .
-  
-  Inductive _elim_rel relc {X Y} RR p src tgt: Prop :=
-  | _elim_rel_intro (SAT: @elim_rel_def relc X Y RR (_elim_rel relc RR) p src tgt).
-
-  Definition elim_rel: forall X Y (RR: X -> Y -> Prop),  bool -> itree hmodE X -> itree hmodE Y -> Prop :=
-     paco6 _elim_rel bot6.
-
-  Variant thread_rel sk0 (cid tid: nat) (fr: Σ) src tgt : Prop :=
-  | thread_rel_init scopes fsp fbody m varg arg
-      (NOC: ~ Nat.eq_dec tid cid)
-      (FR: Own fr ⊢ (ginv sk0 tid) -∗ fsp.(precond) tid m varg arg)
-      (SRC: src = 
-        (interp_hp (HModSem.sandbox scopes (fbody varg)) ε)
-        >>= hp_fun_tail)
-      (TGT: tgt =
-        (interp_hp
-             (HModSem.sandbox scopes (HoareFun (ginv sk0) (stb sk0)
-                  fsp.(precond) fsp.(postcond) fbody arg)) ε) 
-        >>= hp_fun_tail)
-  | thread_rel_body (Q: Any.t -> Any.t -> iProp) p itrS itrT
-      (ELIM: @elim_rel _ _ eq p itrS itrT)
-      (SRC: src = (interp_hp itrS ε) >>= hp_fun_tail)
-      (TGT: tgt =
-        (interp_hp
-            ((if Nat.eq_dec tid cid then Ret tt else trigger (Assume (ginv sk0 tid)));;;
-              vret <- itrT;; 
-              (interp_hpI (prog (SModSem.to_hmod (ginv sk0) (stb sk0) (SMod.modsem md sk0)))
-                ( ret <- trigger (Choose Any.t);;
-                  trigger (Guarantee (Q vret ret));;;
-                  Ret ret))) fr)
-        >>= hp_fun_tail)
-  .
-
-  (* TODO: elim_rel bindC *)
-
-  Lemma elim_rel_def_mon relc relc' X Y RR P P'
-    (RELC: relc <6= relc')
-    (RELI: P <3= P')
-  :
-  @elim_rel_def relc X Y RR P <3= elim_rel_def relc' RR P'.
-  Proof.
-    i. destruct PR; eauto using @elim_rel_def.
-  Qed.
-
-  Lemma elim_rel_tarski elim_rel 
-      X Y RR
-      P
-      (REL: @elim_rel_def elim_rel X Y RR P <3= P)
-    :
-    _elim_rel elim_rel RR <3= P.
-  Proof.
-    fix IH 4. i. inv PR. 
-    inv SAT; eapply REL; try (econs; i; eapply IH; eauto).
-    - econs; eauto.
-    - econs; try refl. i. eapply IH. eauto.
-    - econs 6; eauto. 
-    - econs 7; eauto. 
-    - econs 8; eauto.
-    - econs 9; eauto.
-    - econs 10; eauto.  
-  Qed. 
-
-  Lemma _elim_rel_mon : monotone6 _elim_rel.
-  Proof.
-    ii. eapply elim_rel_tarski; eauto.
-    econs; inv PR.
-    - econs; eauto.
-    - econs 2; eauto.
-    - econs 3; eauto.
-    - econs 4; eauto.
-    - econs 5; eauto.
-    - econs 6; eauto.
-    - econs 7; eauto.
-    - econs 8; eauto.
-    - econs 9; eauto.
-    - econs 10; eauto.
-  Qed.
-
-  Hint Resolve cpn6_wcompat: paco.
-  Hint Resolve _elim_rel_mon: paco.
-  Hint Resolve elim_rel_def_mon: paco.
-
-  Definition elim_rel_indC elim_rel {X Y} RR :=
-    @elim_rel_def bot6 X Y RR (elim_rel X Y RR).
-  
-  Lemma elim_rel_indC_mon: monotone6 elim_rel_indC.
-  Proof.
-    ii. inv IN. 
-    - econs. eauto.
-    - econs. eauto.
-    - econs. eauto.
-    - econs. eauto.
-    - econs; eauto.
-    - econs 6; eauto.
-    - econs 7; eauto.
-    - econs 8; eauto.
-    - econs 9; eauto.
-    - econs 10. eauto.
-  Qed.
-
-  Hint Resolve elim_rel_indC_mon: paco.
-
-  Lemma elim_rel_indC_spec:
-    elim_rel_indC <7= gupaco6 _elim_rel (cpn6 _elim_rel).
-  Proof.
-    eapply wrespect6_uclo; eauto with paco.
-    econs; eauto with paco. i. inv PR; econs.
-    - econs; eauto.
-    - econs; eauto. eapply _elim_rel_mon; eauto. i. econs; eauto.
-    - econs; eauto. eapply _elim_rel_mon; eauto. i. econs; eauto.
-    - econs; eauto. i. eapply _elim_rel_mon; eauto. i. econs; eauto.
-    - econs; eauto. i. eapply _elim_rel_mon; eauto. i. econs; eauto.
-    - econs 6; eauto. i. eapply _elim_rel_mon; eauto. i. econs; eauto.
-    - econs 7; eauto. 
-    - econs 8; eauto. i. eapply _elim_rel_mon; eauto. i. econs; eauto.
-    - econs 9; eauto. i. eapply _elim_rel_mon; eauto. i. econs; eauto.
-    - ss.
-  Qed.
-
-  Lemma _elim_rel_flag_mon X Y RR r (p p': bool) src tgt
-    (REL: @_elim_rel r X Y RR p src tgt)
-    (LE: p -> p')
-    :
-    @_elim_rel r X Y RR p' src tgt.
-  Proof.
-    move REL before r. revert_until REL.
-    pattern p, src, tgt. eapply elim_rel_tarski, REL.
-    i. econs. inv PR.
-    - econs. eauto.
-    - econs; eauto.
-    - econs; eauto.
-    - econs; eauto.
-    - econs; eauto.
-    - econs 6; eauto.
-    - econs 7; eauto.
-    - econs 8; eauto.
-    - econs 9; eauto.
-    - hexploit LE; eauto. i. destruct p'; try discriminate.
-      econs 10; eauto.
-  Qed.
-
-  Lemma elim_rel_flag_mon X Y RR (p p': bool) src tgt
-      (REL: @elim_rel X Y RR p src tgt)
-      (LE: p -> p')
-    :
-    elim_rel RR p' src tgt.
-  Proof.
-    move REL before ms_tgt. revert_until REL. pcofix CIH. i.
-    pstep. eapply _elim_rel_flag_mon; eauto.
-    eapply paco6_mon_bot in REL; eauto. punfold REL.
-  Qed. 
-
-  Variant elim_rel_flagC
-    (r: forall X Y (RR: X -> Y -> Prop) , bool -> itree hmodE X -> itree hmodE Y -> Prop)
-    X Y RR p src tgt : Prop := 
-  | elim_rel_flagC_intro
-    p0
-    (REL: r X Y RR p0 src tgt)
-    (FLAG: p0 = true -> p = true)
-  .
-
-  Lemma elim_rel_flagC_mon r1 r2 (LE: r1 <6= r2) :
-    elim_rel_flagC r1 <6= elim_rel_flagC r2.
-  Proof.
-    ii. destruct PR; econs; eauto.
-  Qed.
-
-  Hint Resolve elim_rel_flagC_mon.
-
-  Lemma elim_rel_flagC_spec:
-    elim_rel_flagC <7= gupaco6 _elim_rel (cpn6 _elim_rel).
-  Proof.
-    eapply wrespect6_uclo; eauto with paco.
-    econs; eauto with paco. i. inv PR.
-    eapply _elim_rel_flag_mon; eauto.
-    eapply _elim_rel_mon. 2: { i. econs. eauto. }
-    eapply GF; eauto.
-  Qed. 
-
-  Variant elim_rel_bindC
-    (r: forall X Y (RR: X -> Y -> Prop), bool -> itree hmodE X -> itree hmodE Y -> Prop)
-    : forall X Y (RR: X -> Y -> Prop), bool -> itree hmodE X -> itree hmodE Y -> Prop
-    :=
-  | elim_rel_bindC_intro
-      Q0 Q1 QQ p i_src i_tgt
-      (REL: r Q0 Q1 QQ p i_src i_tgt)
-
-      X Y RR k_src k_tgt
-      (RELK: ∀vs vt (EQ: QQ vs vt), r X Y RR false (k_src vs) (k_tgt vt))
-    :
-    elim_rel_bindC r RR p (i_src >>= k_src) (i_tgt >>= k_tgt)
-  .
-
-  Lemma elim_rel_bindC_mon
-        r1 r2 
-        (LEr: r1 <6= r2)
-    :
-    elim_rel_bindC r1 <6= elim_rel_bindC r2
-  .
-  Proof.
-    ii. destruct PR; econs; eauto.
-  Qed.
-
-  Lemma elim_rel_bindC_wrespectful:
-    wrespectful6 _elim_rel elim_rel_bindC.
-  Proof.
-    econs; eauto using elim_rel_bindC_mon. i.
-    destruct PR. apply GF in REL.
-    move REL before GF. revert_until REL.
-    pattern p, i_src, i_tgt.
-    eapply elim_rel_tarski, REL. i. 
-    inv PR; grind. 
-    (* eauto 7 using elim_rel_mon, elim_rel_def, rclo3. *)
-    - eapply _elim_rel_mon; cycle 1.
-      { i. econs. eauto. }
-      eapply _elim_rel_flag_mon; eauto.
-      discriminate.
-    - econs. econs. eauto.
-    - econs. econs. eauto.
-    - econs. econs. eauto.
-    - econs. econs 5; eauto; cycle 1.
-      { instantiate (1 := fun _v => _). refl.  }
-      s; eauto.
-    - econs. econs 6; eauto; cycle 1.
-      { instantiate (1 := fun _v => _). refl.  }
-      s; eauto.
-    - econs. econs 7; eauto. 
-    - econs. econs 8; eauto. i. s. eauto. 
-    - econs. econs 9; eauto. i. s. eauto.
-    - econs. econs 10; eauto. 
-      econs 2; eauto. econs; i; econs; eauto.
-  Qed.
-
-  Lemma elim_rel_bindC_spec:
-    elim_rel_bindC <7= gupaco6 _elim_rel (cpn6 _elim_rel).
-  Proof.
-    i. eapply wrespect6_uclo; eauto with paco. eapply elim_rel_bindC_wrespectful.
-  Qed.
-
-
-  Lemma HoareSpawn_sandbox
-      scopes ginv' f fn args
-    :
-    HModSem.sandbox scopes (HoareSpawn ginv' f fn args) = HoareSpawn ginv' f fn args.
-  Proof.
-    unfold HoareSpawn.
-    rewrite/__ HModSB.transl_bind HModSB.transl_core. f_equal. extensionalities.
-    rewrite/__ HModSB.transl_bind HModSB.transl_core. f_equal. extensionalities.
-    rewrite/__ HModSB.transl_bind HModSB.transl_sch. f_equal. extensionalities.
-    rewrite/__ HModSB.transl_bind HModSB.transl_ag. f_equal. extensionalities.
-    rewrite HModSB.transl_ret. ss.
-  Qed. 
-
-  Lemma HoareSpawn_hpI
-      prog ginv' f fn args ktr
-    :
-    interp_hpI prog (HoareSpawn ginv' f fn args >>= ktr)
-    =
-    x <- HoareSpawnE ginv' f fn args;; interp_hpI prog (ktr x).
-  Proof.
-    unfold HoareSpawn, HoareSpawnE. ired.
-    rewrite HIRed.bind_core. f_equal. extensionalities. ired. do 2 f_equal.
-    rewrite HIRed.bind_core. f_equal. extensionalities. ired. do 2 f_equal.
-    rewrite HIRed.bind_sch. f_equal. extensionalities. ired. do 2 f_equal.
-    rewrite HIRed.bind_ag. f_equal.
-  Qed.
-  
-  Lemma HoareYield_sandbox
-      scopes ginv' tid
-    :
-    HModSem.sandbox scopes (HoareYield ginv' tid) = HoareYield ginv' tid.
-  Proof.
-    unfold HoareYield.
-    rewrite/__ HModSB.transl_bind HModSB.transl_ag. f_equal. extensionalities.
-    rewrite/__ HModSB.transl_bind HModSB.transl_sch. f_equal. extensionalities.
-    rewrite/__ HModSB.transl_bind HModSB.transl_sch. f_equal. extensionalities.
-    rewrite HModSB.transl_ag. ss.
-  Qed. 
-
-  Lemma HoareYield_hpI
-      prog ginv' tid ktr
-    :
-    interp_hpI prog (HoareYield ginv' tid >>= ktr)
-    =
-    x <- HoareYieldE ginv' tid;; tau;; interp_hpI prog (ktr x).
-  Proof. 
-    unfold HoareYield, HoareYieldE. ired.
-    rewrite HIRed.bind_ag. f_equal. extensionalities. ired. do 2 f_equal.
-    rewrite HIRed.bind_sch. f_equal. extensionalities. ired. do 2 f_equal.
-    rewrite HIRed.bind_sch. f_equal. extensionalities. ired. do 2 f_equal.
-    rewrite HIRed.bind_ag. f_equal.
-  Qed.
-
-  Lemma HoareCall_inline_aux
-      sk0 scopes fn varg scp fsp fbody 
-      (FIND: alist_find fn (SModSem.fnsems (SMod.modsem md sk0)) = Some (scp, {|fsb_fspec := fsp; fsb_body := fbody|}))
-    :
-    interp_hpI (prog (SModSem.to_hmod (ginv sk0) (stb sk0) (SMod.modsem md sk0))) (HModSem.sandbox scopes (HoareCall fsp fn varg))
-    =
-    (* head *)
-    my_tid <- trigger Tid;; tau;;
-    m <- trigger (Choose (meta fsp));; tau;;
-    arg <- trigger (Choose Any.t);; tau;;
-    trigger (Guarantee (precond fsp my_tid m varg arg));;; tau;; tau;;
-    my_tid' <- trigger Tid;; tau;;
-    m' <- trigger (Take (meta fsp));; tau;;
-    varg' <- trigger (Take Any.t);; tau;;
-    trigger (Assume (precond fsp my_tid' m' varg' arg));;; tau;; 
-    (* body *)
-    vret' <- interp_hpI (prog (SModSem.to_hmod (ginv sk0) (stb sk0) (SMod.modsem md sk0))) 
-                       (HModSem.sandbox scp (interp_smod (ginv sk0) (stb sk0) (fbody varg')));;
-    (* tail *)
-    ret <- trigger (Choose Any.t);; tau;;
-    trigger (Guarantee (postcond fsp my_tid' m' vret' ret));;; tau;; tau;; tau;;
-    vret <- trigger (Take Any.t);; tau;;
-    trigger (Assume (postcond fsp my_tid m vret ret));;; tau;;
-    Ret vret.
-  Proof.
-    unfold HoareCall.
-    (* head *)
-    rewrite/__ HModSB.transl_bind HModSB.transl_sch HIRed.bind_sch. 
-    f_equal. extensionality my_tid. do 2 f_equal.
-    rewrite/__ HModSB.transl_bind HModSB.transl_core HIRed.bind_core.
-    f_equal. extensionality m. do 2 f_equal.
-    rewrite/__ HModSB.transl_bind HModSB.transl_core HIRed.bind_core.
-    f_equal. extensionality arg. do 2 f_equal.
-    rewrite/__ HModSB.transl_bind HModSB.transl_ag HIRed.bind_ag.
-    f_equal. extensionalities. do 2 f_equal.
-    rewrite/__ HModSB.transl_bind HModSB.transl_call HIRed.call.
-    do 2 f_equal. ired.
-    rewrite/__ alist_find_map_snd FIND. ired.
-    unfold HModSem.sandbox_body, interp_sb_hp, HoareFun. s.
-    rewrite/__ HModSB.transl_bind HModSB.transl_sch. ired. rewrite HIRed.bind_sch.
-    f_equal. extensionality my_tid'. do 2 f_equal.
-    rewrite/__ HModSB.transl_bind HModSB.transl_core. ired. rewrite HIRed.bind_core.
-    f_equal. extensionality m'. do 2 f_equal.
-    rewrite/__ HModSB.transl_bind HModSB.transl_core. ired. rewrite HIRed.bind_core.
-    f_equal. extensionality varg'. do 2 f_equal.
-    rewrite/__ HModSB.transl_bind HModSB.transl_ag. ired. rewrite HIRed.bind_ag.
-    f_equal. extensionalities. do 2 f_equal. 
-    (* body *)
-    rewrite HModSB.transl_bind. ired. rewrite HIRed.bind.
-    f_equal. extensionality vret'.
-    rewrite/__ HModSB.transl_bind HModSB.transl_core. ired. rewrite HIRed.bind_core.
-    f_equal. extensionality ret. do 2 f_equal. 
-    rewrite/__ HModSB.transl_bind HModSB.transl_ag. ired. rewrite HIRed.bind_ag.
-    f_equal. extensionalities. do 2 f_equal.
-    rewrite HModSB.transl_ret. ired. rewrite HIRed.tau.
-    do 4 f_equal.
-    rewrite/__ HModSB.transl_bind HModSB.transl_core. ired. rewrite HIRed.bind_core.
-    f_equal. extensionality vret. do 2 f_equal.
-    rewrite/__ HModSB.transl_bind HModSB.transl_ag. ired. rewrite HIRed.bind_ag.
-    f_equal. extensionalities. do 2 f_equal.
-    rewrite/__ HModSB.transl_ret HIRed.ret. ss.
-  Qed.
-
-  Lemma HoareCall_inline
-      sk0 scopes fn varg scp fsp fbody 
-      (FIND: alist_find fn (SModSem.fnsems (SMod.modsem md sk0)) = Some (scp, {|fsb_fspec := fsp; fsb_body := fbody|}))
-    :
-    interp_hpI (prog (SModSem.to_hmod (ginv sk0) (stb sk0) (SMod.modsem md sk0))) (HModSem.sandbox scopes (HoareCall fsp fn varg))
-    =
-    (* head *)
-    '((my_tid, x, my_tid', x'), varg') <- (@hmod_elim_head (meta fsp) (precond fsp) varg);;
-    (* body *)
-    vret' <- interp_hpI (prog (SModSem.to_hmod (ginv sk0) (stb sk0) (SMod.modsem md sk0))) 
-                       (HModSem.sandbox scp (interp_smod (ginv sk0) (stb sk0) (fbody varg')));;
-    (* tail *)
-    @hmod_elim_tail (meta fsp) (postcond fsp) (my_tid, x, my_tid', x') vret'. 
-  Proof.
-    erewrite HoareCall_inline_aux; eauto.
-    unfold hmod_elim_head, hmod_elim_tail. ired. 
-    repeat (f_equal; extensionalities; ired; repeat f_equal). 
-  Qed.
-
-  Definition elim_head_body 
-    sk0 scp fsp fbody varg
-    :=
-    ('((my_tid, x, my_tid', x'), varg') <- (@hmod_elim_head (meta fsp) (precond fsp) varg);;
-    (* body *)
-    vret' <- interp_hpI (prog (SModSem.to_hmod (ginv sk0) (stb sk0) (SMod.modsem md sk0))) 
-                       (HModSem.sandbox scp (interp_smod (ginv sk0) (stb sk0) (fbody varg')));;
-    Ret ((my_tid, x, my_tid', x'), vret')).
-
-  Lemma HoareCall_inline2
-      sk0 scopes fn varg scp fsp fbody 
-      (FIND: alist_find fn (SModSem.fnsems (SMod.modsem md sk0)) = Some (scp, {|fsb_fspec := fsp; fsb_body := fbody|}))
-    :
-    interp_hpI (prog (SModSem.to_hmod (ginv sk0) (stb sk0) (SMod.modsem md sk0))) 
-        (HModSem.sandbox scopes (HoareCall fsp fn varg))
-    =
-    (* head *)
-    RET <- elim_head_body sk0 scp fsp fbody varg;;
-    (* tail *)
-    (fun RET =>
-      let '((my_tid, x, my_tid', x'), vret') := RET in
-      @hmod_elim_tail (meta fsp) (postcond fsp) (my_tid, x, my_tid', x') vret') RET. 
-  Proof.
-    erewrite HoareCall_inline; eauto. unfold elim_head_body. grind.
-  Qed.
-
-  Lemma add_dummy_ret R (itr: itree hmodE R):
-    itr = itr >>= (fun x => Ret x).
-  Proof. grind. Qed.
-
-  Lemma elim_rel_refl
-      sk0 scopes p itr
-      (SKINCL: incl sk sk0)
-      (SKWF: Sk.wf sk0)
-    :
-    @elim_rel _ _ eq p
-      (interp_hpI (prog (SModSemElim.to_elim (SMod.modsem md sk0))) 
-          (HModSem.sandbox scopes itr))
-      (interp_hpI (prog (SModSem.to_hmod (ginv sk0) (stb sk0) (SMod.modsem md sk0))) 
-          (HModSem.sandbox scopes (interp_smod (ginv sk0) (stb sk0) itr))).
-  Proof. 
-    unfold elim_rel.
-    ginit. revert p itr scopes. gcofix CIH. i.
-    assert (CASE:= case_itrH _ itr). des; subst.
-    - rewrite/__ SModRed.interp_ret HModSB.transl_ret !HIRed.ret.
-      gstep. econs. econs; eauto.
-    - rewrite/__ SModRed.interp_tau !HModSB.transl_tau !HIRed.tau.
-      gstep. do 9 econs. econs 10. gbase. eapply CIH; eauto.
-    - rewrite/__ SModRed.interp_bind SModRed.interp_ag !HModSB.transl_bind HModSB.transl_ag. ired.
-      rewrite/__ !HIRed.bind_ag. gstep. do 6 econs.  
-      rewrite/__ HModSB.transl_tau HModSB.transl_ret. ired. 
-      rewrite HIRed.tau. do 5 econs. econs 10. gbase. eapply CIH; eauto.
-    - rewrite/__ SModRed.interp_bind SModRed.interp_ag !HModSB.transl_bind HModSB.transl_ag. ired.
-      rewrite/__ !HIRed.bind_ag. gstep. do 6 econs. 
-      rewrite/__ HModSB.transl_tau HModSB.transl_ret. ired. 
-      rewrite HIRed.tau. do 5 econs. econs 10. gbase. eapply CIH; eauto.
-    - rewrite/__ SModRed.interp_bind SModRed.interp_sch !HModSB.transl_bind HModSB.transl_sch. ired.
-      unfold handle_schE_hmodE. depdes s.
-      + destruct (stb sk0 fn) eqn:STB; ired; cycle 1.
-        { 
-          unfold triggerNB. ired. 
-          rewrite/__ HModSB.transl_bind HModSB.transl_core. ired. 
-          rewrite HIRed.bind_core. gstep. econs. econs 7; ss.
-        }
-        rewrite/__ HoareSpawn_sandbox HoareSpawn_hpI HIRed.bind_sch.
-        gstep. econs. econs 8; eauto. i. s. econs. econs. 
-        rewrite/__ HModSB.transl_tau HModSB.transl_ret. ired. 
-        rewrite HIRed.tau. do 5 econs. econs 10. gbase. eapply CIH; eauto.
-      + rewrite/__ HoareYield_sandbox HoareYield_hpI HIRed.bind_sch.
-        gstep. econs. econs 9; eauto. i. s.
-        rewrite/__ HModSB.transl_tau HModSB.transl_ret. ired. 
-        rewrite HIRed.tau. do 9 econs. econs 10. gbase. eapply CIH; eauto.
-      + rewrite/__ HModSB.transl_sch !HIRed.bind_sch.
-        gstep. do 6 econs.
-        rewrite/__ HModSB.transl_tau HModSB.transl_ret. ired.
-        rewrite HIRed.tau. do 5 econs. econs 10. gbase. eapply CIH; eauto.
-    - rewrite/__ SModRed.interp_bind SModRed.interp_call.
-      unfold handle_callE_hmodE. depdes c. 
-      destruct (stb sk0 fn) eqn: STB; ired; cycle 1.
-      { 
-        unfold triggerNB. 
-        rewrite/__ !HModSB.transl_bind HModSB.transl_core. ired. 
-        rewrite HIRed.bind_core. gstep. econs. econs 7; ss.
-      }
-      do 2 rewrite HModSB.transl_bind. 
-      rewrite/__ HModSB.transl_call HIRed.call HIRed.bind.
-      guclo elim_rel_indC_spec. econs. s.
-      assert (FIND := stb_in_alist_find).
-      specialize (FIND sk0 fn f SKINCL SKWF STB). des.
-      destruct (alist_find fn (List.map (map_snd (λ ksb : list string * fspecbody, (ksb.1, fsb_body ksb.2))) (SModSem.fnsems (SMod.modsem md sk0)))) eqn: FINDS; cycle 1.
-      { exfalso. rewrite/__ alist_find_map_snd FIND in FINDS. clarify.  }
-      ired. destruct p0. rewrite/__ alist_find_map_snd FIND in FINDS. s in FINDS. inv FINDS.
-      unfold HModSem.sandbox_body. s. rewrite HIRed.bind. 
-      erewrite HoareCall_inline2; eauto. 
-      rewrite bind_bind. guclo elim_rel_bindC_spec. econs.
-      {
-        instantiate (1:= fun vs vt => vs = vt.2).
-        unfold elim_head_body. guclo elim_rel_indC_spec. econs 5; swap 1 3.
-        { f_equal. instantiate (1:= fun _ => _). refl. }
-        { instantiate (1:= fun _ => _). refl. }
-        grind. rewrite/__ [interp_hpI _ _]add_dummy_ret. 
-        guclo elim_rel_bindC_spec. econs.
-        { gstep. econs. econs 10. gbase. eapply CIH; ss. }
-        i. gstep. econs. econs. ss.
-      }
-      i. guclo elim_rel_indC_spec.
-      destruct vt, p0, p0, p0. (* Should have "vs = t" in here, lost in bindC *)
-      econs 6; swap 1 3.
-      { f_equal. refl. }
-      { refl. }
-      i. ired. rewrite/__ HModSB.transl_tau !HIRed.tau. 
-      gstep. do 9 econs. econs 10. gbase. ss. subst. eapply CIH; eauto.
-    - depdes s.
-      + rewrite/__ SModRed.interp_bind SModRed.interp_pg !HModSB.transl_bind HModSB.transl_put. ired.
-        des_ifs.
-        * rewrite/__ !HIRed.bind_pg. gstep. do 6 econs.  
-          rewrite/__ HModSB.transl_tau HModSB.transl_ret. ired. 
-          rewrite HIRed.tau. do 5 econs. econs 10. gbase. eapply CIH; eauto.
-        * rewrite/__ !HIRed.bind_core. gstep. do 6 econs.  
-          rewrite/__ HModSB.transl_tau HModSB.transl_ret. ired. 
-          rewrite HIRed.tau. do 5 econs. econs 10. gbase. eapply CIH; eauto.
-      + rewrite/__ SModRed.interp_bind SModRed.interp_pg !HModSB.transl_bind HModSB.transl_get. ired.
-        des_ifs.
-        * rewrite/__ !HIRed.bind_pg. gstep. do 6 econs.  
-          rewrite/__ HModSB.transl_tau HModSB.transl_ret. ired. 
-          rewrite HIRed.tau. do 5 econs. econs 10. gbase. eapply CIH; eauto.
-        * rewrite/__ !HIRed.bind_core. gstep. do 6 econs.  
-          rewrite/__ HModSB.transl_tau HModSB.transl_ret. ired. 
-          rewrite HIRed.tau. do 5 econs. econs 10. gbase. eapply CIH; eauto.
-    - rewrite/__ SModRed.interp_bind SModRed.interp_core !HModSB.transl_bind HModSB.transl_core. ired.
-      rewrite/__ !HIRed.bind_core. gstep. do 6 econs.  
-      rewrite/__ HModSB.transl_tau HModSB.transl_ret. ired. 
-      rewrite HIRed.tau. do 5 econs. econs 10. gbase. eapply CIH; eauto.
-  Qed.
 
   Ltac hide_l := let IT := fresh "ITREE" in
     match goal with 
@@ -807,7 +63,7 @@ Section CANCEL.
 
   Ltac st := prep; guclo simg_indC_spec; econs; try instantiate (1:= smj_top).
   Ltac _iter := rewrite unfold_iter_eq; ired.
-  Ltac _iterI := rewrite/__ [ITree.iter (Cancel.handle_callE _) _]unfold_iter_eq; ired.
+  Ltac _iterI := rewrite/__ [ITree.iter (handle_callE _) _]unfold_iter_eq; ired.
   Ltac _tau := rewrite/__ !StRed.interp_tau.
   Ltac _core := rewrite/__ StRed.interp_bind StRed.interp_core; prep.
   Ltac _coreH := rewrite/__ HModSB.transl_bind HModSB.transl_core interp_hp_bind interp_hp_core; prep.
@@ -822,7 +78,6 @@ Section CANCEL.
 
   Ltac _coreA := _core; st; i; st; grind; _tau; st.
   Ltac _coreE x := _core; st; exists x; st; grind; _tau; st.
-
 
   Inductive Forall3i X Y Z (R: nat -> X -> Y -> Z -> Prop): nat -> list X -> list Y -> list Z -> Prop :=
   | Forall3i_nil i: Forall3i R i [] [] []
@@ -876,6 +131,26 @@ Section CANCEL.
       @Forall3i X Y Z R i xs ys zs. 
   Proof. Admitted.
 
+  Variant thread_rel sk0 (cid tid: nat) (fr: Σ) src tgt : Prop :=
+  | thread_rel_init scopes fsp fbody m varg arg
+      (NOC: ~ Nat.eq_dec tid cid)
+      (FR: Own fr ⊢ (ginv sk0 tid) -∗ fsp.(precond) tid m varg arg)
+      (SRC: src = interp_hp (HModSem.sandbox scopes (fbody varg)))
+      (TGT: tgt = interp_hp (HModSem.sandbox scopes (HoareFun (ginv sk0) (stb sk0)
+                    fsp.(precond) fsp.(postcond) fbody arg)))
+  | thread_rel_body (Q: Any.t -> Any.t -> iProp) p itrS itrT
+      (ELIM: elim_rel ginv stb md _ _ eq p itrS itrT)
+      (SRC: src = interp_hp itrS)
+      (TGT: tgt =
+        (interp_hp
+            ((if Nat.eq_dec tid cid then Ret tt else trigger (Assume (ginv sk0 tid)));;;
+              vret <- itrT;; 
+              (inline_hp (prog (SModSem.to_hmod (ginv sk0) (stb sk0) (SMod.modsem md sk0)))
+                ( ret <- trigger (Choose Any.t);;
+                  trigger (Guarantee (Q vret ret));;;
+                  Ret ret)))))
+  .
+
   (* Lemma wf_fold_lookup cid (mr fr: Σ) frs
         (LEN: cid < strings.length frs)
         (WF: URA.wf (mr ⋅ foldl (λ r1 r2 : Σ, r1 ⋅ r2) ε frs))
@@ -900,20 +175,21 @@ Section CANCEL.
     
     instantiate (1:= ).  *)
 
-  (* Let progS sk0 r :=  ModSem.prog (HModSem.to_mod (SModSemElim.to_elim (SMod.modsem md sk0)) r). *)
+  (* Let progS sk0 r :=  ModSem.prog (HModSem.to_mod (SModSemAux.to_hmod (SMod.modsem md sk0)) r). *)
   (* Let progT sk0 r :=  ModSem.prog (HModSem.to_mod (SModSem.to_hmod (ginv sk0) (stb sk0) (SMod.modsem md sk0)) r). *)
 
 
 
   
   Lemma cancel_aux sk0 (SKINCL: incl sk sk0) (SKWF: Sk.wf sk0):
-    ∀ rs frs mr srcs tgts ps pt cid st
+    ∀ rs frs fr mr srcs tgts ps pt cid st
        (* progS progT
-       (PRS: progS = ModSem.prog (HModSem.to_mod (SModSemElim.to_elim (SMod.modsem md sk0)) rs))
+       (PRS: progS = ModSem.prog (HModSem.to_mod (SModSemAux.to_hmod (SMod.modsem md sk0)) rs))
        (PRT: progT = ModSem.prog (HModSem.to_mod (SModSem.to_hmod (ginv sk0) (stb sk0) (SMod.modsem md sk0)) (rs ⋅ mr))) *)
-       (WF: URA.wf rs)       
+       (WF: ✓ rs)       
        (LEN: cid < List.length frs)
-       (WF: URA.wf (rs ⋅ mr ⋅ (foldl (fun r1 r2 => r1 ⋅ r2) ε frs)))
+       (FR: fr ≡ (foldl (fun r1 r2 => r1 ⋅ r2) ε frs))
+       (WF: ✓ (rs ⋅ mr ⋅ fr))
        (* (RET: ∀fsp m vret ret (MAIN: stb sk0 "CCR_init" = Some fsp), (fsp.(postcond) 0 m vret ret -∗ ⌜vret = ret⌝)) *)
        (REL: Forall3i (thread_rel sk0 cid) 0 frs srcs tgts),
        gpaco7 _simg (cpn7 _simg) bot7 bot7 Any.t Any.t eq ps pt
@@ -924,8 +200,8 @@ Section CANCEL.
                  (* (progS sk0 rs)) *)
                  (ModSem.prog
                     (HModSem.to_mod
-                       (HModSemAux.to_elimI
-                         (SModSemElim.to_elim (SMod.modsem md sk0))) rs)))
+                       (HModSemAux.inline
+                         (SModSemAux.to_hmod (SMod.modsem md sk0))) rs)))
               (cid, srcs))
          (Any.pair st rs↑);; Ret x.2)
          (x <-
@@ -935,13 +211,13 @@ Section CANCEL.
                 (* (progT sk0 (rs ⋅ mr))) *)
                  (ModSem.prog
                     (HModSem.to_mod
-                       (HModSemAux.to_elimI
+                       (HModSemAux.inline
                          (SModSem.to_hmod (ginv sk0) 
                             (stb sk0) (SMod.modsem md sk0))) (rs ⋅ mr)))) 
               (cid, tgts))
-         (Any.pair st (rs ⋅ mr)↑);; Ret x.2).
+         (Any.pair st (fr ⋅ (rs ⋅ mr))↑);; Ret x.2).
   Proof.
-    gcofix CIH. i.
+    (* gcofix CIH. i.
     exploit Forall3i_nth; eauto. i. des.
     rename x into fr, y into src, z into tgt.
     depdes x3.
@@ -954,7 +230,7 @@ Section CANCEL.
     rewrite/__ x1 x2. s. grind.
     punfold ELIM. 
     pattern p, itrS, itrT. eapply elim_rel_tarski, ELIM. i.
-    clear ELIM.
+    clear ELIM. *)
   Admitted.
     (* { *)
       (* hide_r. grind.  *)
@@ -1044,44 +320,74 @@ Section CANCEL.
     (* { admit. } *)
 
   (* Admitted. *)
-  
-  Lemma wf_mon_solve (a b c: Σ) :
-    URA.wf a -> a = b ⋅ c -> URA.wf b.
+
+  Lemma fsb_find_spec fn l fsp fbody (sk0: Sk.t)
+    (SKINCL: incl sk sk0) 
+    (SKWF: Sk.wf sk0) 
+    (FIND: alist_find fn (sbtb SKINCL SKWF) = Some (l, {|fsb_fspec := fsp; fsb_body := fbody|}))
+  :
+    alist_find fn (_stb SKINCL SKWF) = Some (l, fsp).
   Proof.
-    i. inv H0. eapply URA.wf_mon; eauto.
+    unfold sbtb, _stb.
+    rewrite/__ alist_find_map_snd/o_map FIND. ss.
+  Qed. 
+
+  Lemma stb_find_fsb fn fsp l fspec fbody (sk0: Sk.t)
+    (SKINCL: incl sk sk0) 
+    (SKWF: Sk.wf sk0) 
+    (STB: stb sk0 fn = Some fsp)
+    (FIND: alist_find fn (sbtb SKINCL SKWF) = Some (l, {|fsb_fspec:= fspec; fsb_body := fbody|}))
+  :
+    fsp = fspec.
+  Proof.
+    specialize (STBCOMPLETE SKINCL SKWF fn).
+    eapply fsb_find_spec, STBCOMPLETE in FIND; ss.
+    rewrite FIND in STB. inv STB. ss. 
+  Qed.
+
+  Lemma valid_solve (a b c: Σ) :
+    ✓ a -> a ≡  b ⋅ c -> ✓ b.
+  Proof.
+    i. eapply cmra_valid_op_l. setoid_rewrite <- H0. eauto.
+  Qed.
+
+  Lemma valid_solve_eq (a b : Σ) :
+    ✓ a -> a ≡ b -> ✓ b.
+  Proof.
+    i. rewrite <- H0. eauto.
   Qed.
 
   Theorem cancellation Ps Pt
     (COND: forall sk0 (EQV: Sk.equiv sk sk0) (SKWF: Sk.wf sk0), 
       exists fsp m rt,
         (stb sk0 "CCR_init" = Some fsp) /\
-        (forall rs (WF: URA.wf rs) (SRC: Own rs -∗ (Ps sk0)), URA.wf (rs ⋅ rt)) /\ 
+        (forall rs (WF: ✓ rs) (SRC: Own rs ⊢ (Ps sk0)), ✓ (rs ⋅ rt)) /\ 
         (Own rt ⊢ (Pt sk0) ∗ (fsp.(precond) 0 m tt↑ tt↑)) /\
         (∀ m vret ret, (fsp.(postcond) 0 m vret ret) -∗ ⌜vret = ret⌝)
     )
   :
-    refines (md_elim, Ps) (md_tgt, Pt).
+    refines (md_src, Ps) (md_tgt, Pt).
   Proof.
     econs. { s. r. refl. }
     ii. ss. specialize (COND sk0 EQV SKWF). des.
     (* resoure *)
     specialize (COND0 rs WFR SRC).
-    eapply iProp_sepconj in COND1; cycle 1. 
-    { eapply (@wf_mon_solve (rs ⋅ rt) _ rs); [eauto|r_solve]. }
+    eapply Own_split in COND1; cycle 1. 
+    { eapply cmra_valid_op_r. eauto. }
     des. subst.
-    exists (rs ⋅ p). esplits; eauto. 
-    { eapply (@wf_mon_solve (rs ⋅ (p ⋅ q)) _ q); [eauto|r_solve]. }
-    { iIntros "[_ P]". iStopProof. eapply iProp_Own; eauto. }
+    exists (rs ⋅ a1). esplits; eauto.
+    { eapply (@valid_solve (rs ⋅ rt) _ a2); r_solve; eauto. } 
+    { iIntros "[_ P]". iStopProof. eauto. }
     {
       inv WFM. econs; eauto.
       rewrite/SModSem.to_hmod !map_map_compose !fst_map_snd.
-      rewrite/SModSemElim.to_elim !map_map_compose !fst_map_snd in wf_fns. 
+      rewrite/SModSemAux.to_hmod !map_map_compose !fst_map_snd in wf_fns. 
       ss.
     }
     r. eapply adequacy_global_itree.
     instantiate (1:= smj_top).
     instantiate (1:= smj_top).
-    unfold ModSem.initial_itr. s. unfold ITree.map.
+    unfold ModSem.compile. s. unfold ITree.map.
     (* remember (alist_encode (SModSem.initial_st (SMod.modsem md sk0))) as st. *)
     destruct (alist_find "CCR_init" (SModSem.fnsems (SMod.modsem md sk0))) eqn:E; cycle 1.
     {
@@ -1089,7 +395,7 @@ Section CANCEL.
       unfold interp_modE at 2.
       rewrite/interp_schE_callE unfold_iter_eq /handle_schE_callE.
       grind. rewrite/__ StRed.interp_bind. grind.
-      destruct (resum IFun void (Choose void)) eqn:V.
+      destruct (resum IFun False (Choose False)) eqn:V.
       { inv V. }
       depdes c; inv V. resub.
       rewrite/__ [interp_stateE _ _ _]StRed.interp_core. grind.
@@ -1097,12 +403,11 @@ Section CANCEL.
     }
     rewrite/__ !alist_find_map/o_map E. s. 
     erewrite !wrap_elimI_well_scoped; cycle 1.
-    { unfold SModSem.to_hmod. s. rewrite alist_find_map_snd. rewrite E. ss. }
-    { unfold SModSemElim.to_elim. s. rewrite alist_find_map_snd. rewrite E. ss. }
-    ired.
-    destruct p0. s.
+    { unfold SModSem.to_hmod. s. rewrite alist_find_map_snd. instantiate (1:= "CCR_init"). rewrite E. ss. }
+    { unfold SModSemAux.to_hmod. s. rewrite alist_find_map_snd. instantiate (1:= "CCR_init"). rewrite E. ss. }
+    ired. destruct p. s.
     unfold HModSem.sandbox_body, interp_hp_fun. s.
-    unfold interp_hpI_fun, interp_sb_hp, interp_hp_body. s.
+    unfold inline_hp_fun, interp_sb_hp. s.
     unfold HoareFun.
     
     unfold interp_modE, interp_schE_callE. 
@@ -1125,30 +430,33 @@ Section CANCEL.
     _iter. _tau. st. st. st.
     rewrite interp_hp_tau. _iter. _tau. st. st.
     rewrite/__ HModSB.transl_bind HModSB.transl_ag HIRed.bind_ag interp_hp_bind interp_hp_Assume. ired.
-    _iter. _core. st. exists q. st. ired. _tau. st. 
+    _iter. _core. st. exists a2. st. ired. _tau. st. 
     _iter. _sget. ired. _tau. st. st.
     hss. ired. hss. ired.
     _iter. _core. st.
-    assert (URA.wf (q ⋅ ε ⋅ (rs ⋅ p))). 
-    { eapply wf_eq_solve; [eapply COND0|r_solve]. }
+    assert (✓ (a2 ⋅ (rs ⋅ a1))). 
+    { 
+      eapply (@valid_solve _ _ ε COND0). r_solve.
+      setoid_rewrite COND1. r_solve.
+    }
     exists H. ired. _tau. st. st. 
-    _iter. _core. st.
-    eapply iProp_Own in COND4. exists COND4. ired.
-    _iter. _tau. do 4 st.
-    rewrite interp_hp_tau. _iter. _tau. st. st.
+    _iter. _core. st. exists COND4. ired.
+    _iter. _tau. st. st. _supd. _iter. _supd.
+    _iter. _tau. st. st. rewrite interp_hp_tau. _iter. _tau. st. st.
     
     (* CCR_main's precond all executed. *)
     reveal ITREE. 
     eapply cancel_aux; eauto.
-    { instantiate (1:= [_]). ss. }
-    { s. eapply wf_eq_solve; [eapply H|r_solve]. }
+    { instantiate (1:= [a2]). ss. }
+    { s. r_solve. }
+    { eapply (valid_solve_eq H). r_solve. }
     econs; eauto using Forall3i.
     econs 2; s; eauto; cycle 1. 
     {
       rewrite/__ HModSB.transl_bind HIRed.bind. 
       instantiate (1:= postcond fsb_fspec 0 m).
-      instantiate (1:= interp_hpI _ (HModSem.sandbox l (interp_smod (ginv sk0) (stb sk0) (fsb_body tt↑)))).
-      ired. repeat f_equal; [|r_solve]. 
+      instantiate (1:= inline_hp _ (HModSem.sandbox l (interp_smod (ginv sk0) (stb sk0) (fsb_body tt↑)))).
+      ired. repeat f_equal. 
       extensionalities.
       rewrite/__ HModSB.transl_bind HModSB.transl_core. do 2 f_equal.
       extensionalities.
