cancellation/ElimRel.v
@@ -1,0 +1,663 @@
+Require Import Coqlib.
+Require Import Behavior.
+Require Import AList.
+Require Import SMod2HMod SMod2HModAux.
+Require Import Skeleton.
+Require Import PCM IPM.
+Require Import Any.
+Require Export STB.
+Require Import ModSim ISim HPSim.
+Require Import CtxRefine CtxRefineFacts MainAdequacy ClosedAdequacy.
+Require Import SimGlobal SimGlobalFacts.
+Require Import SMod HMod Mod Events.
+Require Import HModInline Cancel.
+
+Section REL.
+  Context `{Σ: GRA.t}.
+  Variable ginv: Sk.t -> invspec.
+  Variable stb: Sk.t -> gname -> option fspec.
+  Variable md: SMod.t.
+  Notation iProp := (iProp Σ).
+  Let sk: Sk.t := SMod.sk md.
+
+  Definition hmod_elim_head X P : Any.t -> itree hmodE ((nat * X * nat * X) * Any.t)
+    :=
+    fun varg =>
+      my_tid <- trigger Tid;; tau;;
+      x <- trigger (Choose X);; tau;;
+      arg <- trigger (Choose Any.t);; tau;;
+      trigger (Guarantee (P my_tid x varg arg));;; tau;; tau;;
+      my_tid' <- trigger Tid;; tau;;
+      x' <- trigger (Take X);; tau;;
+      varg' <- trigger (Take _);; tau;;
+      trigger (Assume (P my_tid' x' varg' arg));;; tau;;
+      Ret ((my_tid, x, my_tid', x'), varg').
+
+  Definition hmod_elim_tail X Q : (nat * X * nat * X) -> Any.t -> itree hmodE Any.t
+    :=
+    fun '(my_tid, x, my_tid', x') vret' =>
+      ret <- trigger (Choose Any.t);; tau;;
+      trigger (Guarantee (Q my_tid' x' vret' ret));;; tau;; tau;; tau;;
+      vret <- trigger (Take Any.t);; tau;;
+      trigger (Assume (Q my_tid x vret ret));;; tau;;
+      Ret vret.
+      
+  Definition HoareSpawnE ginv' (fsp: fspec) (fn: gname) (arg: Any.t) : itree hmodE nat :=
+    x <- trigger (Choose fsp.(meta));; tau;;
+    varg <- trigger (Choose Any.t);; tau;;
+    tid <- trigger (Spawn fn arg);; tau;;
+    trigger (Guarantee (ginv' tid -∗ fsp.(precond) tid x arg varg));;; tau;;
+    Ret tid.
+
+  Definition HoareYieldE ginv' (tid: nat) : itree hmodE unit :=
+    trigger (Guarantee (ginv' tid));;; tau;;
+    trigger (Yield tid);;; tau;;
+    my_tid <- trigger Tid;; tau;;
+    trigger (Assume (ginv' my_tid)).
+
+  Variant elim_rel_def
+    (relc: forall X Y (RR: X -> Y -> Prop), bool -> itree hmodE X -> itree hmodE Y -> Prop)
+    {X Y}
+    (RR: X -> Y -> Prop)
+    (reli: bool -> itree hmodE X -> itree hmodE Y -> Prop)
+    : bool -> itree hmodE X -> itree hmodE Y -> Prop
+  :=
+  | elim_rel_base v0 v1 p
+    (RET: RR v0 v1)
+    :
+    elim_rel_def relc RR reli p (Ret v0) (Ret v1)
+
+  | elim_rel_tau_src p itrS itrT
+      (ITR: reli true itrS itrT)
+    :
+    elim_rel_def relc RR reli p (tau;; itrS) (itrT)
+
+  | elim_rel_tau_tgt p itrS itrT
+      (ITR: reli true itrS itrT)
+    :
+    elim_rel_def relc RR reli p (itrS) (tau;; itrT)
+
+  | elim_rel_add {R} p itr ktrS ktrT
+      (KTR: forall (v: R), reli true (ktrS v) (ktrT v))
+    :
+    elim_rel_def relc RR reli p (itr >>= ktrS) (itr >>= ktrT)
+
+  | elim_rel_head X P p v src tgt ktrS ktrT
+      (KTR: forall m, reli true (ktrS v) (ktrT (m, v)))
+      (EQS: src = ktrS v)
+      (EQT: tgt = (@hmod_elim_head X P v) >>= ktrT)
+    :
+    elim_rel_def relc RR reli p src tgt
+                  
+  | elim_rel_tail X Q m v p src tgt ktrS ktrT
+      (KTR: reli true (ktrS v) (ktrT v))
+      (EQS: src = ktrS v)
+      (EQT: tgt = (@hmod_elim_tail X Q m v) >>= ktrT)
+    :
+    elim_rel_def relc RR reli p src tgt
+
+  | elim_rel_NB
+      p src tgt itrS ktrT
+      (EQS: src = itrS)
+      (EQT: tgt = trigger (Choose False) >>= ktrT)
+    :
+    elim_rel_def relc RR reli p src tgt
+
+   | elim_rel_spawn
+      sk0 p src tgt f fn args ktrS ktrT
+      (SKINCL: incl sk sk0)
+      (SKWF: Sk.wf sk0)
+      (STB: stb sk0 fn = Some f)
+      (KTR: forall x, reli true (ktrS x) (ktrT x))
+      (EQS: src =  trigger (Spawn fn args) >>= ktrS)
+      (EQT: tgt = HoareSpawnE (ginv sk0) f fn args >>= ktrT)
+    :
+    elim_rel_def relc RR reli p src tgt
+
+  | elim_rel_yield
+      sk0 tid p src tgt ktrS ktrT
+      (SKINCL: incl sk sk0)
+      (SKWF: Sk.wf sk0)
+      (KTR: forall x, reli true (ktrS x) (ktrT x))
+      (EQS: src = trigger (Yield tid) >>= ktrS)
+      (EQT: tgt = HoareYieldE (ginv sk0) tid >>= ktrT)
+    :
+    elim_rel_def relc RR reli p src tgt
+
+  | elim_rel_progress
+      src tgt
+      (REL: relc X Y RR false src tgt)
+    :
+    elim_rel_def relc RR reli true src tgt 
+  .
+  
+  Inductive _elim_rel relc {X Y} RR p src tgt: Prop :=
+  | _elim_rel_intro (SAT: @elim_rel_def relc X Y RR (_elim_rel relc RR) p src tgt).
+
+  Definition elim_rel: forall X Y (RR: X -> Y -> Prop),  bool -> itree hmodE X -> itree hmodE Y -> Prop :=
+     paco6 _elim_rel bot6.
+
+  Lemma elim_rel_def_mon relc relc' X Y RR P P'
+    (RELC: relc <6= relc')
+    (RELI: P <3= P')
+  :
+  @elim_rel_def relc X Y RR P <3= elim_rel_def relc' RR P'.
+  Proof.
+    i. destruct PR; eauto using @elim_rel_def.
+  Qed.
+
+  Lemma elim_rel_tarski elim_rel 
+      X Y RR
+      P
+      (REL: @elim_rel_def elim_rel X Y RR P <3= P)
+    :
+    _elim_rel elim_rel RR <3= P.
+  Proof.
+    fix IH 4. i. inv PR. 
+    inv SAT; eapply REL; try (econs; i; eapply IH; eauto).
+    - econs; eauto.
+    - econs; try refl. i. eapply IH. eauto.
+    - econs 6; eauto. 
+    - econs 7; eauto. 
+    - econs 8; eauto.
+    - econs 9; eauto.
+    - econs 10; eauto.  
+  Qed. 
+
+  Lemma _elim_rel_mon : monotone6 _elim_rel.
+  Proof.
+    ii. eapply elim_rel_tarski; eauto.
+    econs; inv PR.
+    - econs; eauto.
+    - econs 2; eauto.
+    - econs 3; eauto.
+    - econs 4; eauto.
+    - econs 5; eauto.
+    - econs 6; eauto.
+    - econs 7; eauto.
+    - econs 8; eauto.
+    - econs 9; eauto.
+    - econs 10; eauto.
+  Qed.
+
+  Hint Resolve cpn6_wcompat: paco.
+  Hint Resolve _elim_rel_mon: paco.
+  Hint Resolve elim_rel_def_mon: paco.
+
+  Definition elim_rel_indC elim_rel {X Y} RR :=
+    @elim_rel_def bot6 X Y RR (elim_rel X Y RR).
+  
+  Lemma elim_rel_indC_mon: monotone6 elim_rel_indC.
+  Proof.
+    ii. inv IN. 
+    - econs. eauto.
+    - econs. eauto.
+    - econs. eauto.
+    - econs. eauto.
+    - econs; eauto.
+    - econs 6; eauto.
+    - econs 7; eauto.
+    - econs 8; eauto.
+    - econs 9; eauto.
+    - econs 10. eauto.
+  Qed.
+
+  Hint Resolve elim_rel_indC_mon: paco.
+
+  Lemma elim_rel_indC_spec:
+    elim_rel_indC <7= gupaco6 _elim_rel (cpn6 _elim_rel).
+  Proof.
+    eapply wrespect6_uclo; eauto with paco.
+    econs; eauto with paco. i. inv PR; econs.
+    - econs; eauto.
+    - econs; eauto. eapply _elim_rel_mon; eauto. i. econs; eauto.
+    - econs; eauto. eapply _elim_rel_mon; eauto. i. econs; eauto.
+    - econs; eauto. i. eapply _elim_rel_mon; eauto. i. econs; eauto.
+    - econs; eauto. i. eapply _elim_rel_mon; eauto. i. econs; eauto.
+    - econs 6; eauto. i. eapply _elim_rel_mon; eauto. i. econs; eauto.
+    - econs 7; eauto. 
+    - econs 8; eauto. i. eapply _elim_rel_mon; eauto. i. econs; eauto.
+    - econs 9; eauto. i. eapply _elim_rel_mon; eauto. i. econs; eauto.
+    - ss.
+  Qed.
+
+  Lemma _elim_rel_flag_mon X Y RR r (p p': bool) src tgt
+    (REL: @_elim_rel r X Y RR p src tgt)
+    (LE: p -> p')
+    :
+    @_elim_rel r X Y RR p' src tgt.
+  Proof.
+    move REL before r. revert_until REL.
+    pattern p, src, tgt. eapply elim_rel_tarski, REL.
+    i. econs. inv PR.
+    - econs. eauto.
+    - econs; eauto.
+    - econs; eauto.
+    - econs; eauto.
+    - econs; eauto.
+    - econs 6; eauto.
+    - econs 7; eauto.
+    - econs 8; eauto.
+    - econs 9; eauto.
+    - hexploit LE; eauto. i. destruct p'; try discriminate.
+      econs 10; eauto.
+  Qed.
+
+  Lemma elim_rel_flag_mon X Y RR (p p': bool) src tgt
+      (REL: @elim_rel X Y RR p src tgt)
+      (LE: p -> p')
+    :
+    elim_rel X Y RR p' src tgt.
+  Proof.
+    move REL before Y. revert_until REL. pcofix CIH. i.
+    pstep. eapply _elim_rel_flag_mon; eauto.
+    eapply paco6_mon_bot in REL; eauto. punfold REL.
+  Qed. 
+
+  Variant elim_rel_flagC
+    (r: forall X Y (RR: X -> Y -> Prop) , bool -> itree hmodE X -> itree hmodE Y -> Prop)
+    X Y RR p src tgt : Prop := 
+  | elim_rel_flagC_intro
+    p0
+    (REL: r X Y RR p0 src tgt)
+    (FLAG: p0 = true -> p = true)
+  .
+
+  Lemma elim_rel_flagC_mon r1 r2 (LE: r1 <6= r2) :
+    elim_rel_flagC r1 <6= elim_rel_flagC r2.
+  Proof.
+    ii. destruct PR; econs; eauto.
+  Qed.
+
+  Hint Resolve elim_rel_flagC_mon.
+
+  Lemma elim_rel_flagC_spec:
+    elim_rel_flagC <7= gupaco6 _elim_rel (cpn6 _elim_rel).
+  Proof.
+    eapply wrespect6_uclo; eauto with paco.
+    econs; eauto with paco. i. inv PR.
+    eapply _elim_rel_flag_mon; eauto.
+    eapply _elim_rel_mon. 2: { i. econs. eauto. }
+    eapply GF; eauto.
+  Qed. 
+
+  Variant elim_rel_bindC
+    (r: forall X Y (RR: X -> Y -> Prop), bool -> itree hmodE X -> itree hmodE Y -> Prop)
+    : forall X Y (RR: X -> Y -> Prop), bool -> itree hmodE X -> itree hmodE Y -> Prop
+    :=
+  | elim_rel_bindC_intro
+      Q0 Q1 QQ p i_src i_tgt
+      (REL: r Q0 Q1 QQ p i_src i_tgt)
+
+      X Y RR k_src k_tgt
+      (RELK: ∀vs vt (EQ: QQ vs vt), r X Y RR false (k_src vs) (k_tgt vt))
+    :
+    elim_rel_bindC r X Y RR p (i_src >>= k_src) (i_tgt >>= k_tgt)
+  .
+
+  Lemma elim_rel_bindC_mon
+        r1 r2 
+        (LEr: r1 <6= r2)
+    :
+    elim_rel_bindC r1 <6= elim_rel_bindC r2
+  .
+  Proof.
+    ii. destruct PR; econs; eauto.
+  Qed.
+
+  Lemma elim_rel_bindC_wrespectful:
+    wrespectful6 _elim_rel elim_rel_bindC.
+  Proof.
+    econs; eauto using elim_rel_bindC_mon. i.
+    destruct PR. apply GF in REL.
+    move REL before GF. revert_until REL.
+    pattern p, i_src, i_tgt.
+    eapply elim_rel_tarski, REL. i. 
+    inv PR; grind. 
+    (* eauto 7 using elim_rel_mon, elim_rel_def, rclo3. *)
+    - eapply _elim_rel_mon; cycle 1.
+      { i. econs. eauto. }
+      eapply _elim_rel_flag_mon; eauto.
+      discriminate.
+    - econs. econs. eauto.
+    - econs. econs. eauto.
+    - econs. econs. eauto.
+    - econs. econs 5; eauto; cycle 1.
+      { instantiate (1 := fun _v => _). refl.  }
+      s; eauto.
+    - econs. econs 6; eauto; cycle 1.
+      { instantiate (1 := fun _v => _). refl.  }
+      s; eauto.
+    - econs. econs 7; eauto. 
+    - econs. econs 8; eauto. i. s. eauto. 
+    - econs. econs 9; eauto. i. s. eauto.
+    - econs. econs 10; eauto. 
+      econs 2; eauto. econs; i; econs; eauto.
+  Qed.
+
+  Lemma elim_rel_bindC_spec:
+    elim_rel_bindC <7= gupaco6 _elim_rel (cpn6 _elim_rel).
+  Proof.
+    i. eapply wrespect6_uclo; eauto with paco. eapply elim_rel_bindC_wrespectful.
+  Qed.
+
+End REL.
+
+Hint Resolve cpn6_wcompat: paco.
+Hint Resolve _elim_rel_mon: paco.
+
+
+Section CANCEL.
+  Context `{Σ: GRA.t}.
+  Variable ginv: Sk.t -> invspec.
+  Variable stb: Sk.t -> gname -> option fspec.
+  Variable md: SMod.t.
+  Notation iProp := (iProp Σ).
+  Let sk: Sk.t := SMod.sk md.
+  Let ms (sk0: Sk.t) (SKINCL: incl sk sk0) (SKWF: Sk.wf sk0) := 
+    SMod.modsem md sk0.
+  Let sbtb (sk0: Sk.t) (SKINCL: incl sk sk0) (SKWF: Sk.wf sk0): alist gname (list string * fspecbody) := 
+    (ms sk0 SKINCL SKWF).(SModSem.fnsems).
+  Let _stb (sk0: Sk.t) (SKINCL: incl sk sk0) (SKWF: Sk.wf sk0): alist gname (list string * fspec) := 
+    List.map (map_snd (fun '(fn, fs) => (fn, fs.(fsb_fspec)))) (sbtb sk0 SKINCL SKWF).
+
+  Hypothesis STBCOMPLETE:
+    forall 
+      sk0 (SKINCL: incl sk sk0) (SKWF: Sk.wf sk0)
+      fn scfsp (FIND: alist_find fn (_stb sk0 SKINCL SKWF) = Some scfsp), stb sk0 fn = Some scfsp.2.
+  Hypothesis STBSOUND:
+    forall 
+      sk0 (SKINCL: incl sk sk0) (SKWF: Sk.wf sk0)
+      fn (FIND: alist_find fn (_stb sk0 SKINCL SKWF) = None),
+      (<<NONE: stb sk0 fn = None>>).
+
+  Lemma stb_in_alist_find
+        (sk0: Sk.t) fn fsp
+        (SKINCL: incl sk sk0) 
+        (SKWF: Sk.wf sk0)
+        (SOME: stb sk0 fn = Some fsp)
+      :
+        exists l fbody, 
+          alist_find fn (SModSem.fnsems (SMod.modsem md sk0)) = Some (l, {|fsb_fspec :=fsp; fsb_body := fbody|}).
+  Proof.
+    destruct (alist_find fn (_stb sk0 SKINCL SKWF)) eqn: FIND; cycle 1.
+    { eapply STBSOUND in FIND. des. clarify. }
+    unfold _stb, sbtb, ms in FIND.
+    rewrite/__ alist_find_map_snd/o_map in FIND. des_ifs.
+    destruct p0, f. exists l, fsb_body. repeat f_equal.
+    assert (alist_find fn (_stb sk0 SKINCL SKWF) = Some (l, fsb_fspec)).
+    { rewrite/_stb alist_find_map_snd /o_map /sbtb /ms Heq. ss. }
+    eapply STBCOMPLETE in H. ss. rewrite SOME in H. inv H. ss.
+  Qed.
+
+  Lemma HoareSpawn_sandbox
+      scopes ginv' f fn args
+    :
+    HModSem.sandbox scopes (HoareSpawn ginv' f fn args) = HoareSpawn ginv' f fn args.
+  Proof.
+    unfold HoareSpawn.
+    rewrite/__ HModSB.transl_bind HModSB.transl_core. f_equal. extensionalities.
+    rewrite/__ HModSB.transl_bind HModSB.transl_core. f_equal. extensionalities.
+    rewrite/__ HModSB.transl_bind HModSB.transl_sch. f_equal. extensionalities.
+    rewrite/__ HModSB.transl_bind HModSB.transl_ag. f_equal. extensionalities.
+    rewrite HModSB.transl_ret. ss.
+  Qed. 
+
+  Lemma HoareSpawn_hpI
+      prog ginv' f fn args ktr
+    :
+    inline_hp prog (HoareSpawn ginv' f fn args >>= ktr)
+    =
+    x <- HoareSpawnE ginv' f fn args;; inline_hp prog (ktr x).
+  Proof.
+    unfold HoareSpawn, HoareSpawnE. ired.
+    rewrite HIRed.bind_core. f_equal. extensionalities. ired. do 2 f_equal.
+    rewrite HIRed.bind_core. f_equal. extensionalities. ired. do 2 f_equal.
+    rewrite HIRed.bind_sch. f_equal. extensionalities. ired. do 2 f_equal.
+    rewrite HIRed.bind_ag. f_equal.
+  Qed.
+  
+  Lemma HoareYield_sandbox
+      scopes ginv' tid
+    :
+    HModSem.sandbox scopes (HoareYield ginv' tid) = HoareYield ginv' tid.
+  Proof.
+    unfold HoareYield.
+    rewrite/__ HModSB.transl_bind HModSB.transl_ag. f_equal. extensionalities.
+    rewrite/__ HModSB.transl_bind HModSB.transl_sch. f_equal. extensionalities.
+    rewrite/__ HModSB.transl_bind HModSB.transl_sch. f_equal. extensionalities.
+    rewrite HModSB.transl_ag. ss.
+  Qed. 
+
+  Lemma HoareYield_hpI
+      prog ginv' tid ktr
+    :
+    inline_hp prog (HoareYield ginv' tid >>= ktr)
+    =
+    x <- HoareYieldE ginv' tid;; tau;; inline_hp prog (ktr x).
+  Proof. 
+    unfold HoareYield, HoareYieldE. ired.
+    rewrite HIRed.bind_ag. f_equal. extensionalities. ired. do 2 f_equal.
+    rewrite HIRed.bind_sch. f_equal. extensionalities. ired. do 2 f_equal.
+    rewrite HIRed.bind_sch. f_equal. extensionalities. ired. do 2 f_equal.
+    rewrite HIRed.bind_ag. f_equal.
+  Qed.
+
+  Lemma HoareCall_inline_aux
+      sk0 scopes fn varg scp fsp fbody 
+      (FIND: alist_find fn (SModSem.fnsems (SMod.modsem md sk0)) = Some (scp, {|fsb_fspec := fsp; fsb_body := fbody|}))
+    :
+    inline_hp (prog (SModSem.to_hmod (ginv sk0) (stb sk0) (SMod.modsem md sk0))) (HModSem.sandbox scopes (HoareCall fsp fn varg))
+    =
+    (* head *)
+    my_tid <- trigger Tid;; tau;;
+    m <- trigger (Choose (meta fsp));; tau;;
+    arg <- trigger (Choose Any.t);; tau;;
+    trigger (Guarantee (precond fsp my_tid m varg arg));;; tau;; tau;;
+    my_tid' <- trigger Tid;; tau;;
+    m' <- trigger (Take (meta fsp));; tau;;
+    varg' <- trigger (Take Any.t);; tau;;
+    trigger (Assume (precond fsp my_tid' m' varg' arg));;; tau;; 
+    (* body *)
+    vret' <- inline_hp (prog (SModSem.to_hmod (ginv sk0) (stb sk0) (SMod.modsem md sk0))) 
+                       (HModSem.sandbox scp (interp_smod (ginv sk0) (stb sk0) (fbody varg')));;
+    (* tail *)
+    ret <- trigger (Choose Any.t);; tau;;
+    trigger (Guarantee (postcond fsp my_tid' m' vret' ret));;; tau;; tau;; tau;;
+    vret <- trigger (Take Any.t);; tau;;
+    trigger (Assume (postcond fsp my_tid m vret ret));;; tau;;
+    Ret vret.
+  Proof.
+    unfold HoareCall.
+    (* head *)
+    rewrite/__ HModSB.transl_bind HModSB.transl_sch HIRed.bind_sch. 
+    f_equal. extensionality my_tid. do 2 f_equal.
+    rewrite/__ HModSB.transl_bind HModSB.transl_core HIRed.bind_core.
+    f_equal. extensionality m. do 2 f_equal.
+    rewrite/__ HModSB.transl_bind HModSB.transl_core HIRed.bind_core.
+    f_equal. extensionality arg. do 2 f_equal.
+    rewrite/__ HModSB.transl_bind HModSB.transl_ag HIRed.bind_ag.
+    f_equal. extensionalities. do 2 f_equal.
+    rewrite/__ HModSB.transl_bind HModSB.transl_call HIRed.call.
+    do 2 f_equal. ired.
+    rewrite/__ alist_find_map_snd FIND. ired.
+    unfold HModSem.sandbox_body, interp_sb_hp, HoareFun. s.
+    rewrite/__ HModSB.transl_bind HModSB.transl_sch. ired. rewrite HIRed.bind_sch.
+    f_equal. extensionality my_tid'. do 2 f_equal.
+    rewrite/__ HModSB.transl_bind HModSB.transl_core. ired. rewrite HIRed.bind_core.
+    f_equal. extensionality m'. do 2 f_equal.
+    rewrite/__ HModSB.transl_bind HModSB.transl_core. ired. rewrite HIRed.bind_core.
+    f_equal. extensionality varg'. do 2 f_equal.
+    rewrite/__ HModSB.transl_bind HModSB.transl_ag. ired. rewrite HIRed.bind_ag.
+    f_equal. extensionalities. do 2 f_equal. 
+    (* body *)
+    rewrite HModSB.transl_bind. ired. rewrite HIRed.bind.
+    f_equal. extensionality vret'.
+    rewrite/__ HModSB.transl_bind HModSB.transl_core. ired. rewrite HIRed.bind_core.
+    f_equal. extensionality ret. do 2 f_equal. 
+    rewrite/__ HModSB.transl_bind HModSB.transl_ag. ired. rewrite HIRed.bind_ag.
+    f_equal. extensionalities. do 2 f_equal.
+    rewrite HModSB.transl_ret. ired. rewrite HIRed.tau.
+    do 4 f_equal.
+    rewrite/__ HModSB.transl_bind HModSB.transl_core. ired. rewrite HIRed.bind_core.
+    f_equal. extensionality vret. do 2 f_equal.
+    rewrite/__ HModSB.transl_bind HModSB.transl_ag. ired. rewrite HIRed.bind_ag.
+    f_equal. extensionalities. do 2 f_equal.
+    rewrite/__ HModSB.transl_ret HIRed.ret. ss.
+  Qed.
+
+  Lemma HoareCall_inline
+      sk0 scopes fn varg scp fsp fbody 
+      (FIND: alist_find fn (SModSem.fnsems (SMod.modsem md sk0)) = Some (scp, {|fsb_fspec := fsp; fsb_body := fbody|}))
+    :
+    inline_hp (prog (SModSem.to_hmod (ginv sk0) (stb sk0) (SMod.modsem md sk0))) (HModSem.sandbox scopes (HoareCall fsp fn varg))
+    =
+    (* head *)
+    '((my_tid, x, my_tid', x'), varg') <- (hmod_elim_head (meta fsp) (precond fsp) varg);;
+    (* body *)
+    vret' <- inline_hp (prog (SModSem.to_hmod (ginv sk0) (stb sk0) (SMod.modsem md sk0))) 
+                       (HModSem.sandbox scp (interp_smod (ginv sk0) (stb sk0) (fbody varg')));;
+    (* tail *)
+    hmod_elim_tail (meta fsp) (postcond fsp) (my_tid, x, my_tid', x') vret'. 
+  Proof.
+    erewrite HoareCall_inline_aux; eauto.
+    unfold hmod_elim_head, hmod_elim_tail. ired. 
+    repeat (f_equal; extensionalities; ired; repeat f_equal). 
+  Qed.
+
+  Definition elim_head_body 
+    sk0 scp fsp fbody varg
+    :=
+    ('((my_tid, x, my_tid', x'), varg') <- (hmod_elim_head (meta fsp) (precond fsp) varg);;
+    (* body *)
+    vret' <- inline_hp (prog (SModSem.to_hmod (ginv sk0) (stb sk0) (SMod.modsem md sk0))) 
+                       (HModSem.sandbox scp (interp_smod (ginv sk0) (stb sk0) (fbody varg')));;
+    Ret ((my_tid, x, my_tid', x'), vret')).
+
+  Lemma HoareCall_inline2
+      sk0 scopes fn varg scp fsp fbody 
+      (FIND: alist_find fn (SModSem.fnsems (SMod.modsem md sk0)) = Some (scp, {|fsb_fspec := fsp; fsb_body := fbody|}))
+    :
+    inline_hp (prog (SModSem.to_hmod (ginv sk0) (stb sk0) (SMod.modsem md sk0))) 
+        (HModSem.sandbox scopes (HoareCall fsp fn varg))
+    =
+    (* head *)
+    RET <- elim_head_body sk0 scp fsp fbody varg;;
+    (* tail *)
+    (fun RET =>
+      let '((my_tid, x, my_tid', x'), vret') := RET in
+      hmod_elim_tail (meta fsp) (postcond fsp) (my_tid, x, my_tid', x') vret') RET. 
+  Proof.
+    erewrite HoareCall_inline; eauto. unfold elim_head_body. grind.
+  Qed.
+
+  Lemma add_dummy_ret R (itr: itree hmodE R):
+    itr = itr >>= (fun x => Ret x).
+  Proof. grind. Qed.
+
+  Lemma elim_rel_refl
+      sk0 scopes p itr
+      (SKINCL: incl sk sk0)
+      (SKWF: Sk.wf sk0)
+    :
+    elim_rel ginv stb md _ _ eq p
+      (inline_hp (prog (SModSemAux.to_hmod (SMod.modsem md sk0))) 
+          (HModSem.sandbox scopes itr))
+      (inline_hp (prog (SModSem.to_hmod (ginv sk0) (stb sk0) (SMod.modsem md sk0))) 
+          (HModSem.sandbox scopes (interp_smod (ginv sk0) (stb sk0) itr))).
+  Proof. 
+    unfold elim_rel.
+    ginit. revert p itr scopes. gcofix CIH. i.
+    assert (CASE:= case_itrH _ itr). des; subst.
+    - rewrite/__ SModRed.interp_ret HModSB.transl_ret !HIRed.ret.
+      gstep. econs. econs; eauto.
+    - rewrite/__ SModRed.interp_tau !HModSB.transl_tau !HIRed.tau.
+      gstep. do 9 econs. econs 10. gbase. eapply CIH; eauto.
+    - rewrite/__ SModRed.interp_bind SModRed.interp_ag !HModSB.transl_bind HModSB.transl_ag. ired.
+      rewrite/__ !HIRed.bind_ag. gstep. do 6 econs.  
+      rewrite/__ HModSB.transl_tau HModSB.transl_ret. ired. 
+      rewrite HIRed.tau. do 5 econs. econs 10. gbase. eapply CIH; eauto.
+    - rewrite/__ SModRed.interp_bind SModRed.interp_ag !HModSB.transl_bind HModSB.transl_ag. ired.
+      rewrite/__ !HIRed.bind_ag. gstep. do 6 econs. 
+      rewrite/__ HModSB.transl_tau HModSB.transl_ret. ired. 
+      rewrite HIRed.tau. do 5 econs. econs 10. gbase. eapply CIH; eauto.
+    - rewrite/__ SModRed.interp_bind SModRed.interp_sch !HModSB.transl_bind HModSB.transl_sch. ired.
+      unfold handle_schE_hmodE. depdes s.
+      + destruct (stb sk0 fn) eqn:STB; ired; cycle 1.
+        { 
+          unfold triggerNB. ired. 
+          rewrite/__ HModSB.transl_bind HModSB.transl_core. ired. 
+          rewrite HIRed.bind_core. gstep. econs. econs 7; ss.
+        }
+        rewrite/__ HoareSpawn_sandbox HoareSpawn_hpI HIRed.bind_sch.
+        gstep. econs. econs 8; eauto. i. s. econs. econs. 
+        rewrite/__ HModSB.transl_tau HModSB.transl_ret. ired. 
+        rewrite HIRed.tau. do 5 econs. econs 10. gbase. eapply CIH; eauto.
+      + rewrite/__ HoareYield_sandbox HoareYield_hpI HIRed.bind_sch.
+        gstep. econs. econs 9; eauto. i. s.
+        rewrite/__ HModSB.transl_tau HModSB.transl_ret. ired. 
+        rewrite HIRed.tau. do 9 econs. econs 10. gbase. eapply CIH; eauto.
+      + rewrite/__ HModSB.transl_sch !HIRed.bind_sch.
+        gstep. do 6 econs.
+        rewrite/__ HModSB.transl_tau HModSB.transl_ret. ired.
+        rewrite HIRed.tau. do 5 econs. econs 10. gbase. eapply CIH; eauto.
+    - rewrite/__ SModRed.interp_bind SModRed.interp_call.
+      unfold handle_callE_hmodE. depdes c. 
+      destruct (stb sk0 fn) eqn: STB; ired; cycle 1.
+      { 
+        unfold triggerNB. 
+        rewrite/__ !HModSB.transl_bind HModSB.transl_core. ired. 
+        rewrite HIRed.bind_core. gstep. econs. econs 7; ss.
+      }
+      do 2 rewrite HModSB.transl_bind. 
+      rewrite/__ HModSB.transl_call HIRed.call HIRed.bind.
+      guclo elim_rel_indC_spec. econs. s.
+      assert (FIND := stb_in_alist_find).
+      specialize (FIND sk0 fn f SKINCL SKWF STB). des.
+      destruct (alist_find fn (List.map (map_snd (λ ksb : list string * fspecbody, (ksb.1, fsb_body ksb.2))) (SModSem.fnsems (SMod.modsem md sk0)))) eqn: FINDS; cycle 1.
+      { exfalso. rewrite/__ alist_find_map_snd FIND in FINDS. clarify.  }
+      ired. destruct p0. rewrite/__ alist_find_map_snd FIND in FINDS. s in FINDS. inv FINDS.
+      unfold HModSem.sandbox_body. s. rewrite HIRed.bind. 
+      erewrite HoareCall_inline2; eauto. 
+      rewrite bind_bind. guclo elim_rel_bindC_spec. econs.
+      {
+        instantiate (1:= fun vs vt => vs = vt.2).
+        unfold elim_head_body. guclo elim_rel_indC_spec. econs 5; swap 1 3.
+        { f_equal. }
+        { instantiate (1:= fun _ => _). refl. }
+        grind. rewrite/__ [inline_hp _ _]add_dummy_ret. 
+        guclo elim_rel_bindC_spec. econs.
+        { gstep. econs. econs 10. gbase. eapply CIH; ss. }
+        i. gstep. econs. econs. ss.
+      }
+      i. guclo elim_rel_indC_spec.
+      destruct vt, p0, p0, p0. (* Should have "vs = t" in here, lost in bindC *)
+      econs 6; swap 1 3.
+      { f_equal. }
+      { refl. }
+      i. ired. rewrite/__ HModSB.transl_tau !HIRed.tau. 
+      gstep. do 9 econs. econs 10. gbase. ss. subst. eapply CIH; eauto.
+    - depdes s.
+      + rewrite/__ SModRed.interp_bind SModRed.interp_pg !HModSB.transl_bind HModSB.transl_put. ired.
+        des_ifs.
+        * rewrite/__ !HIRed.bind_pg. gstep. do 6 econs.  
+          rewrite/__ HModSB.transl_tau HModSB.transl_ret. ired. 
+          rewrite HIRed.tau. do 5 econs. econs 10. gbase. eapply CIH; eauto.
+        * rewrite/__ !HIRed.bind_core. gstep. do 6 econs.  
+          rewrite/__ HModSB.transl_tau HModSB.transl_ret. ired. 
+          rewrite HIRed.tau. do 5 econs. econs 10. gbase. eapply CIH; eauto.
+      + rewrite/__ SModRed.interp_bind SModRed.interp_pg !HModSB.transl_bind HModSB.transl_get. ired.
+        des_ifs.
+        * rewrite/__ !HIRed.bind_pg. gstep. do 6 econs.  
+          rewrite/__ HModSB.transl_tau HModSB.transl_ret. ired. 
+          rewrite HIRed.tau. do 5 econs. econs 10. gbase. eapply CIH; eauto.
+        * rewrite/__ !HIRed.bind_core. gstep. do 6 econs.  
+          rewrite/__ HModSB.transl_tau HModSB.transl_ret. ired. 
+          rewrite HIRed.tau. do 5 econs. econs 10. gbase. eapply CIH; eauto.
+    - rewrite/__ SModRed.interp_bind SModRed.interp_core !HModSB.transl_bind HModSB.transl_core. ired.
+      rewrite/__ !HIRed.bind_core. gstep. do 6 econs.  
+      rewrite/__ HModSB.transl_tau HModSB.transl_ret. ired. 
+      rewrite HIRed.tau. do 5 econs. econs 10. gbase. eapply CIH; eauto.
+  Qed.
+
+End CANCEL.
