cancellation/HModInline.v
@@ -1,0 +1,241 @@
+Require Import Coqlib.
+Require Import sflib.
+Require Import ITreelib.
+Require Import AList.
+Require Import Behavior.
+Require Import Skeleton.
+Require Import PCM IPM.
+Require Import Any.
+Require Export STB.
+Require Import Events HMod.
+
+Set Implicit Arguments.
+
+
+
+(* Inlining every function call in HMod. *)
+Section INTERP.
+  Context `{Σ: GRA.t}.
+
+  Definition handle_callE (prog: callE ~> itree hmodE): itree hmodE Any.t -> itree hmodE (_ + Any.t)
+  :=
+    fun itr =>
+      match observe (itr: itree hmodE Any.t) with
+      | RetF rv => Ret (inr rv)
+      | TauF itr' => tau;; Ret (inl itr')
+      | VisF (inr1 (inr1 (inr1 (inr1 e)))) k =>
+          v <- trigger e;; Ret (inl (k v))
+      | VisF (inr1 (inr1 (inr1 (inl1 e)))) k => 
+          v <- trigger e;; Ret (inl (k v))
+      | VisF (inr1 (inr1 (inl1 c))) k =>
+          Ret (inl (x <- prog _ c;; tau;; (k x)))
+      | VisF (inr1 (inl1 e)) k =>
+          v <- trigger e;; Ret (inl (k v))
+      | VisF (inl1 e) k =>
+          v <- trigger e;; Ret (inl (k v))
+      end.
+
+  Definition inline_hp (prog: callE ~> itree hmodE) (itr: itree hmodE Any.t)
+    : itree hmodE Any.t
+    :=
+    ITree.iter (handle_callE prog) itr.
+
+  Definition inline_hp_fun (prog: callE ~> itree hmodE) (body: Any.t -> itree hmodE Any.t)
+    : Any.t -> itree hmodE Any.t
+    :=
+    fun args =>
+      inline_hp prog (body args).
+
+  Definition prog (ms: HModSem.t) : callE ~> itree hmodE :=
+    fun _ '(Call fn args) =>
+      lbody <- (alist_find fn ms.(HModSem.fnsems))!;;
+      HModSem.sandbox_body lbody args.
+      
+  Definition inline_hp_fbody (ms: HModSem.t)
+    : (list string * (Any.t -> itree hmodE Any.t)) -> (list string * (Any.t -> itree hmodE Any.t))
+    :=
+    fun '(k, b) => (k, inline_hp_fun (prog ms) b).
+
+  Definition wrap_sandbox scopeS: list string * (Any.t -> itree hmodE Any.t) -> list string * (Any.t -> itree hmodE Any.t)
+    := 
+    fun kb => (scopeS, HModSem.sandbox_body kb).
+
+  Definition wrap_elimI ms: list string * (Any.t -> itree hmodE Any.t) -> list string * (Any.t -> itree hmodE Any.t)
+    :=
+    fun kb => inline_hp_fbody ms (wrap_sandbox ms.(HModSem.scopes) kb). 
+
+End INTERP.
+
+Module HModSemAux.
+  Section AUX.
+    Context `{Σ: GRA.t}.
+    Import HModSem.
+
+    Program Definition inline (ms: HModSem.t): HModSem.t := {|
+      HModSem.scopes := ms.(scopes);
+      HModSem.fnsems := List.map (map_snd (wrap_elimI ms)) (ms.(fnsems));
+      (* HModSem.fnsems := List.map (map_snd (λ ksb, (ksb.1, inline_hp_fun (prog ms) ksb.2))) (ms.(fnsems)); *)
+      HModSem.initial_st := ms.(initial_st);
+    |}.
+    Next Obligation.
+      i. depdes ms. ss. ii. unfold fnsems_scopes in *. unfold map_snd in*.
+      rewrite! alist_find_map in H. unfold o_map in H.
+      des_ifs; ss. 
+      (* inv Heq0.
+      specialize (well_scoped_fns0 fn a).
+      des_ifs; ss. inv Heq. eauto. *)
+    Qed.
+    Next Obligation. ii. destruct ms. ss. eauto. Qed.
+    Next Obligation. ii. destruct ms. ss. eauto. Qed.
+
+    (* Definition to_elim ms := to_hmod ((interp_sb_hp_elim) ∘ fsb_body) ms. *)
+
+  End AUX.
+End HModSemAux.
+
+Module HModAux.
+  Section AUX.
+    Context `{Σ: GRA.t}.
+    Import HMod.
+
+    Definition inline (md: t) := {|
+      HMod.modsem := fun sk => HModSemAux.inline (md.(modsem) sk);
+      HMod.sk := md.(sk);
+    |}.
+
+  End AUX.
+End HModAux.
+
+Module HIRed.
+  Section RED.
+    Context `{Σ: GRA.t}.
+
+    Variable ms: HModSem.t.
+
+    Lemma iter_handle_bind i k:
+      ITree.iter (handle_callE (prog ms)) (i >>= k)
+      =
+      x <- (ITree.iter (handle_callE (prog ms)) i);; ITree.iter (handle_callE (prog ms)) (k x).
+    Proof. 
+      eapply bisim_is_eq.
+      eapply (@gpaco2_init _ _ _ _ (eqitC eq false false)); eauto with paco.
+      revert i k. gcofix CIH. i.
+      ides i.
+      - grind. rewrite/__ [_ _ (Ret _)]unfold_iter_eq. grind.
+        gfinal. right. eapply paco2_mon_bot; eauto.
+        apply Reflexive_eqit. auto.
+      - grind. rewrite! unfold_iter_eq. grind.
+        gstep. econs. gstep. econs. gbase. eapply CIH.
+      - rewrite! unfold_iter_eq.
+        destruct e.
+        {
+          grind. rewrite! bind_trigger. gstep. econs. i.
+          r. grind. gstep. econs. gbase. eauto.
+        }
+        destruct p.
+        {
+          grind. rewrite! bind_trigger. gstep. econs. i.
+          r. grind. gstep. econs. gbase. eauto.  
+        }
+        destruct s.
+        {
+          grind. gstep. econs. 
+          guclo eqit_clo_trans; eauto.
+          econs; cycle 1.
+          { refl. }
+          { gbase. eapply CIH. }
+          { instantiate (1:= eq). i. subst. refl. }
+          { i. subst. refl. }
+          grind. 
+          replace (` x : X <- prog ms c;; (tau;; ITree.subst k (k0 x)))
+          with (` r0 : X <- prog ms c;; ` x : Any.t <- (tau;; k0 r0);; k x) by grind.
+          refl.
+        } 
+        destruct s.
+        {
+          grind. rewrite! bind_trigger. gstep. econs. i.
+          r. grind. gstep. econs. gbase. eauto.
+        }
+        grind. rewrite! bind_trigger. gstep. econs. i.
+        r. grind. gstep. econs. gbase. eauto.
+      Unshelve. eauto with paco.
+    Qed.
+        
+    Lemma ret 
+      prog (x: Any.t)
+    :
+      inline_hp prog (Ret x) = Ret x.
+    Proof.
+      rewrite/inline_hp unfold_iter_eq. grind.
+    Qed.
+
+    Lemma tau
+      prog t
+    :
+      inline_hp prog (tau;; t) = tau;; tau;; inline_hp prog t.
+    Proof.
+      rewrite/inline_hp unfold_iter_eq. grind.
+    Qed.
+
+    Lemma bind
+      itr ktr
+    :
+      inline_hp (prog ms) (itr >>= ktr)
+      =
+      x <- inline_hp (prog ms) itr;; inline_hp (prog ms) (ktr x).
+    Proof.
+      rewrite/inline_hp iter_handle_bind. refl.
+    Qed.
+
+    Lemma bind_sch
+      X prog (e: schE X) ktr
+    :
+      inline_hp prog (x <- trigger e;; ktr x) 
+      =
+      x <- trigger e;; tau;; inline_hp prog (ktr x).
+    Proof.
+      rewrite/inline_hp unfold_iter_eq. grind.
+    Qed.
+
+    Lemma bind_core
+      X prog (e: coreE X) ktr
+    :
+      inline_hp prog (x <- trigger e;; ktr x) 
+      =
+      x <- trigger e;; tau;; inline_hp prog (ktr x).
+    Proof.
+      rewrite/inline_hp unfold_iter_eq. grind.
+    Qed.
+
+    Lemma bind_pg
+      X prog (e: pgE X) ktr
+    :
+      inline_hp prog (x <- trigger e;; ktr x) 
+      =
+      x <- trigger e;; tau;; inline_hp prog (ktr x).
+    Proof.
+      rewrite/inline_hp unfold_iter_eq. grind.
+    Qed.
+
+    Lemma bind_ag
+      X prog (e: agE X) ktr
+    :
+      inline_hp prog (x <- trigger e;; ktr x) 
+      =
+      x <- trigger e;; tau;; inline_hp prog (ktr x).
+    Proof.
+      rewrite/inline_hp unfold_iter_eq. grind.
+    Qed.
+
+    Lemma call
+      prog ktr (fn: string) arg 
+    :
+      inline_hp prog (trigger (Call fn arg) >>= ktr)
+      =
+      tau;; inline_hp prog (x <- prog Any.t (resum IFun Any.t (Call fn arg));; tau;; ITree.subst ktr (Ret x)).
+    Proof.
+      rewrite/inline_hp unfold_iter_eq. ired. refl.
+    Qed.
+
+  End RED.
+End HIRed.
