cancellation/SMod2HModAux.v
@@ -1,0 +1,56 @@
+Require Import Coqlib.
+Require Import sflib.
+Require Import ITreelib.
+Require Import AList.
+Require Import Behavior.
+Require Import Events SMod HMod Mod.
+Require Import SMod2HMod HMod2Mod.
+Require Import Skeleton.
+Require Import PCM IPM.
+Require Import Any.
+Require Export STB.
+Require Import ModSim.
+
+Set Implicit Arguments.
+
+(******* Rename each section into proper name  *******)
+
+
+Module SModSemAux.
+Section AUX.
+  Import SModSem.
+  Context `{Σ: GRA.t}.
+  Variable ginv: invspec.
+  Variable stb: gname -> option fspec.
+
+  Program Definition to_hmod (ms: t): HModSem.t := {|
+    HModSem.scopes := ms.(scopes);
+    HModSem.fnsems := List.map (map_snd (λ ksb, (ksb.1, fsb_body ksb.2))) (ms.(fnsems));
+    HModSem.initial_st := ms.(initial_st);
+  |}.
+  Next Obligation.
+    i. destruct ms. ss. ii. unfold fnsems_scopes in *. unfold map_snd in*.
+    rewrite! alist_find_map in H. specialize (well_scoped_fns0 fn a).
+    des_ifs; ss. inv Heq. eauto.
+  Qed.
+  Next Obligation. ii. destruct ms. ss. eauto. Qed.
+  Next Obligation. ii. destruct ms. ss. eauto. Qed.
+
+End AUX.
+End SModSemAux.
+
+Module SModAux.
+Section AUX.
+  Import SMod.
+  Context `{Σ: GRA.t}.
+  Variable ginv: Sk.t -> invspec.
+  Variable stb: Sk.t -> gname -> option fspec.
+
+  Definition to_hmod (md: t) := {|
+    HMod.modsem := fun sk => SModSemAux.to_hmod (md.(modsem) sk);
+    HMod.sk := md.(sk);
+  |}.
+
+End AUX.
+End SModAux.
+
