cancellation/StRed.v
@@ -1,0 +1,80 @@
+Require Import Coqlib.
+Require Import Behavior.
+Require Import AList.
+Require Import Mod2ITree Events.
+
+Module StRed.
+Section RED.
+
+  Lemma interp_bind
+        A B
+        (itr: itree (stateE +' coreE) A)
+        (ktr: A -> itree (stateE +' coreE) B)
+        st0
+    :
+      interp_stateE B (v <- itr ;; ktr v) st0 =
+      '(st1, v) <- interp_stateE A (itr) st0 ;; interp_stateE B (ktr v) st1.
+  Proof.
+    unfold interp_stateE. grind. destruct x. grind.
+  Qed.
+
+  Lemma interp_tau
+        A (itr: itree (stateE +' coreE) A)
+        st0 
+    :
+      interp_stateE _ (tau;; itr) st0 = tau;; interp_stateE _ itr st0
+  .
+  Proof. 
+    unfold interp_stateE. grind. 
+  Qed.
+
+  Lemma interp_st
+        E st0 T e
+    :
+      @interp_stateE E T (trigger e) st0 =
+      '(st1, r) <- handle_stateE _ e st0;;
+      tau;; Ret (st1, r).
+  Proof.
+    unfold interp_stateE. grind. destruct x. grind.
+  Qed.
+
+  Lemma interp_ret
+        E A st0 v
+    :
+      @interp_stateE E A (Ret v) st0 = Ret (st0, v)
+  .
+  Proof. 
+    unfold interp_stateE. grind.
+  Qed.
+  
+  Lemma interp_core
+        st0 T
+        (e: coreE T)
+    :
+      @interp_stateE (coreE) _ (trigger e) st0 = r <- trigger e;; tau;; Ret (st0, r)
+  .
+  Proof.
+    unfold interp_stateE. grind.
+    unfold Mod2ITree.pure_state. grind.
+  Qed.
+
+  Lemma interp_UB
+        st0 A
+    :
+      (@interp_stateE (stateE +' coreE) A (triggerUB) st0) = triggerUB
+  .
+  Proof.
+    unfold interp_stateE, Mod2ITree.pure_state, triggerUB. grind.
+  Qed.
+  
+  Lemma interp_NB
+        st0 A
+    :
+      (@interp_stateE (stateE +' coreE) A (triggerNB) st0) = triggerNB
+  .
+  Proof.
+    unfold interp_stateE, Mod2ITree.pure_state, triggerNB. grind.
+  Qed.  
+
+End RED.
+End StRed.
